erasure/theories/ERemoveParams.v
@@ -11,7 +11,8 @@ From MetaCoq.PCUIC Require Import PCUICAst PCUICAstUtils
 From MetaCoq.SafeChecker Require Import PCUICWfEnvImpl.
      
 From MetaCoq.Erasure Require Import EAst EAstUtils EInduction EArities Extract Prelim
-    ELiftSubst ESpineView EOptimizePropDiscr ErasureFunction EEtaExpanded ECSubst.
+    ELiftSubst ESpineView EOptimizePropDiscr EGlobalEnv EEnvMap 
+    EWcbvEval ErasureFunction EEtaExpanded ECSubst EWcbvEvalEtaInd.
 
 Local Open Scope string_scope.
 Set Asymmetric Patterns.
@@ -33,6 +34,8 @@ Hint Constructors Ee.eval : core.
 Set Warnings "-notation-overridden".
 Import E.
 Set Warnings "+notation-overridden".
+
+Import MCList (map_InP, map_InP_spec).
 
 Section strip.
   Context (Σ : GlobalContextMap.t).
@@ -190,7 +193,7 @@ Section strip.
     - destruct Nat.compare => //. 
     - specialize (H a k H1 H2).
       rewrite !csubst_mkApps in H2 *.
-      rewrite isEtaExp_mkApps // in H3.
+      rewrite isEtaExp_mkApps_napp // in H3.
       destruct construct_viewc.
       * cbn. rewrite strip_mkApps //.
       * move/andP: H3 => [] et ev.
@@ -204,7 +207,7 @@ Section strip.
           pose proof (decompose_app_notApp _ _ _ eqk).
           assert (l <> []).
           { intros ->. rewrite (decompose_app_inv eqk) in eqa. now rewrite eqa in H5. }
-          rewrite isEtaExp_mkApps // in H4.
+          rewrite isEtaExp_mkApps_napp // in H4.
           assert ((l ++ map (csubst a k) v)%list <> []).
           { destruct l; cbn; congruence. }
 
@@ -285,28 +288,28 @@ Section strip.
     forallb (closedn 0) args ->
     forallb (isEtaExp Σ) args ->
     isEtaExp Σ br.2 ->
-    strip (ETyping.iota_red pars args br) = ETyping.iota_red pars (map strip args) (on_snd strip br).
+    strip (EGlobalEnv.iota_red pars args br) = EGlobalEnv.iota_red pars (map strip args) (on_snd strip br).
   Proof.
     intros cl etaargs etabr.
-    unfold ETyping.iota_red.
+    unfold EGlobalEnv.iota_red.
     rewrite strip_substl //.
     rewrite forallb_rev forallb_skipn //.
     rewrite forallb_rev forallb_skipn //.
     now rewrite map_rev map_skipn.
   Qed.
   
-  Lemma strip_fix_subst mfix : ETyping.fix_subst (map (map_def strip) mfix) = map strip (ETyping.fix_subst mfix).
+  Lemma strip_fix_subst mfix : EGlobalEnv.fix_subst (map (map_def strip) mfix) = map strip (EGlobalEnv.fix_subst mfix).
   Proof.
-    unfold ETyping.fix_subst.
+    unfold EGlobalEnv.fix_subst.
     rewrite map_length.
     generalize #|mfix|.
     induction n; simpl; auto.
     f_equal; auto. now simp strip.
   Qed.
 
-  Lemma strip_cofix_subst mfix : ETyping.cofix_subst (map (map_def strip) mfix) = map strip (ETyping.cofix_subst mfix).
+  Lemma strip_cofix_subst mfix : EGlobalEnv.cofix_subst (map (map_def strip) mfix) = map strip (EGlobalEnv.cofix_subst mfix).
   Proof.
-    unfold ETyping.cofix_subst.
+    unfold EGlobalEnv.cofix_subst.
     rewrite map_length.
     generalize #|mfix|.
     induction n; simpl; auto.
@@ -314,7 +317,7 @@ Section strip.
   Qed.
 
   Lemma strip_cunfold_fix mfix idx n f : 
-    forallb (closedn 0) (ETyping.fix_subst mfix) ->
+    forallb (closedn 0) (EGlobalEnv.fix_subst mfix) ->
     forallb (isEtaExp Σ ∘ dbody) mfix ->
     Ee.cunfold_fix mfix idx = Some (n, f) ->
     Ee.cunfold_fix (map (map_def strip) mfix) idx = Some (n, strip f).
@@ -333,7 +336,7 @@ Section strip.
 
   
   Lemma strip_cunfold_cofix mfix idx n f : 
-    forallb (closedn 0) (ETyping.cofix_subst mfix) ->
+    forallb (closedn 0) (EGlobalEnv.cofix_subst mfix) ->
     forallb (isEtaExp Σ ∘ dbody) mfix ->
     Ee.cunfold_cofix mfix idx = Some (n, f) ->
     Ee.cunfold_cofix (map (map_def strip) mfix) idx = Some (n, strip f).
@@ -364,21 +367,6 @@ Ltac simp_eta := simp isEtaExp; rewrite -?isEtaExp_equation_1.
 Tactic Notation "simp_strip" "in" hyp(H) := simp strip in H; rewrite -?strip_equation_1 in H.
 Ltac simp_strip := simp strip; rewrite -?strip_equation_1.
 
-Definition isEtaExp_constant_decl Σ cb := 
-  option_default (isEtaExp Σ) cb.(cst_body) true.
-
-Definition isEtaExp_decl Σ d :=
-  match d with
-  | ConstantDecl cb => isEtaExp_constant_decl Σ cb
-  | InductiveDecl idecl => true
-  end.
-
-Fixpoint isEtaExp_env (Σ : global_declarations) := 
-  match Σ with 
-  | [] => true
-  | decl :: Σ => isEtaExp_decl Σ decl.2 && isEtaExp_env Σ
-  end.
-
 Definition strip_constant_decl Σ cb := 
   {| cst_body := option_map (strip Σ) cb.(cst_body) |}.
   
@@ -394,10 +382,7 @@ Definition strip_decl Σ d :=
 Definition strip_env Σ :=
   map (on_snd (strip_decl Σ)) Σ.(GlobalContextMap.global_decls).
 
-Import ETyping.
-
-(* Lemma strip_extends Σ Σ' : extends Σ Σ' ->
-  strip Σ t = strip Σ' t. *)
+Import EGlobalEnv.
 
 Lemma lookup_env_strip Σ kn : 
   lookup_env (strip_env Σ) kn = 
@@ -423,74 +408,11 @@ Proof.
   destruct g; simpl; auto. destruct nth_error => //.
 Qed.
 
-Lemma isEtaExp_tApp (Σ : global_context) f u : isEtaExp Σ (mkApps f u) -> 
-  let (hd, args) := decompose_app (mkApps f u) in
-  match construct_viewc hd with
-  | view_construct kn c => isEtaExp_app Σ kn c #|args| && forallb (isEtaExp Σ) args
-  | view_other u discr => isEtaExp Σ hd && forallb (isEtaExp Σ) args
-  end.
-Proof.
-  destruct decompose_app eqn:da.
-  rewrite (decompose_app_inv da).
-  pose proof (decompose_app_notApp _ _ _ da).
-  destruct l. cbn -[isEtaExp].
-  intros eq; rewrite eq.
-  destruct (construct_viewc t) => //. simp isEtaExp in eq; now rewrite eq.
-  assert (t0 :: l <> []) by congruence.
-  revert da H0. generalize (t0 :: l). clear t0 l; intros l.
-  intros da nnil.
-  rewrite isEtaExp_mkApps //.
-Qed.
-
-Lemma eval_construct  {fl : Ee.WcbvFlags} Σ kn c args e : 
-  Ee.eval Σ (mkApps (tConstruct kn c) args) e -> ∑ args', (e = mkApps (tConstruct kn c) args') × All2 (Ee.eval Σ) args args'.
-Proof.
-  revert e; induction args using rev_ind; intros e.
-  - intros ev. depelim ev. exists []=> //.
-  - intros ev. rewrite mkApps_app /= in ev.
-    depelim ev; try solve_discr.
-    destruct (IHargs _ ev1) as [? []]. solve_discr.
-    all:try specialize (IHargs _ ev1) as [? []]; try solve_discr.
-    * subst f'. 
-      exists (x0 ++ [a'])%list.
-      rewrite mkApps_app /= //.
-      cbn in i. split => //. eapply All2_app; eauto.
-    * now cbn in i.
-Qed.
-
-Lemma app_tip_nil {A} (l : list A) (x : A) : (l ++ [x])%list <> [].
-Proof.
-  destruct l; cbn; congruence.
-Qed.
-
-Lemma eval_mkApps_Construct {fl : Ee.WcbvFlags} Σ kn c args args' : 
-  All2 (Ee.eval Σ) args args' ->
-  Ee.eval Σ (mkApps (tConstruct kn c) args) (mkApps (tConstruct kn c) args').
-Proof.
-  revert args'. induction args using rev_ind; intros args'; destruct args' using rev_case; intros a.
-  - depelim a. constructor => //.
-  - depelim a. cbn. now apply app_tip_nil in H.
-  - depelim a. now apply app_tip_nil in H.
-  - eapply All2_app_inv in a as []. 2:{ eapply All2_length in a. len in a. cbn in a. lia. } 
-    depelim a0. clear a0. rewrite !mkApps_app /=.
-    constructor; auto. 
-    rewrite !negb_or isLambda_mkApps // isFixApp_mkApps // isBox_mkApps //.
-Qed.
-
-Definition remove_last {A} (args : list A) := 
-  List.firstn (#|args| - 1) args.
-
-Lemma remove_last_app {A} (l : list A) x : 
-  remove_last (l ++ [x]) = l.
-Proof.
-  unfold remove_last. cbn. len.
-  replace (#|l| + 1 -1) with #|l| by lia.
-  rewrite firstn_app Nat.sub_diag /= firstn_all app_nil_r //.
-Qed.
+Arguments Ee.eval {wfl}.
 
 Arguments isEtaExp : simpl never.
 
-Lemma isEtaExp_tApp' {Σ} {f u} : isEtaExp Σ (tApp f u) -> 
+Lemma isEtaExp_mkApps {Σ} {f u} : isEtaExp Σ (tApp f u) -> 
   let (hd, args) := decompose_app (tApp f u) in
   match construct_viewc hd with
   | view_construct kn c =>
@@ -500,7 +422,7 @@ Lemma isEtaExp_tApp' {Σ} {f u} : isEtaExp Σ (tApp f u) ->
     [&& isEtaExp Σ hd, forallb (isEtaExp Σ) args, isEtaExp Σ f & isEtaExp Σ u]
   end.
 Proof.
-  move/(isEtaExp_tApp Σ f [u]).
+  move/(isEtaExp_mkApps Σ f [u]).
   cbn -[decompose_app]. destruct decompose_app eqn:da.
   destruct construct_viewc eqn:cv => //.
   intros ->.
@@ -531,97 +453,6 @@ Proof.
   now rewrite remove_last_app.
 Qed.
 
-Lemma remove_last_last {A} (l : list A) (a : A) : l <> [] ->
-  l = (remove_last l ++ [last l a])%list.
-Proof.
-  induction l using rev_ind.
-  congruence.
-  intros. rewrite remove_last_app last_last //.
-Qed.
-
-Lemma forallb_repeat {A} {p : A -> bool} {a : A} {n} : 
-  p a ->
-  forallb p (repeat a n).
-Proof.
-  intros pa.
-  induction n; cbn; auto.
-  now rewrite pa IHn.
-Qed.
-
-Lemma isEtaExp_lookup_ext {Σ} {kn d}: 
-  isEtaExp_env Σ ->
-  lookup_env Σ kn = Some d ->
-  ∑ Σ', extends Σ' Σ × isEtaExp_decl Σ' d.
-Proof.
-  induction Σ; cbn.
-  - move=> _; rewrite /declared_constant /lookup_env /= //.
-  - move=> /andP[] etaa etaΣ.
-    destruct a as [kn' d']; cbn in *.
-    rewrite /declared_constant /=.
-    case:eqb_specT => //.
-    * intros e; subst kn'. move=> [=]. intros ->.
-      exists Σ. split => //. now exists [(kn, d)].
-    * intros ne. move=> Hl. destruct (IHΣ etaΣ Hl) as [Σ' [ext eta]].
-      exists Σ'; split => //.
-      destruct ext as [Σ'' ->].
-      now exists ((kn', d')::Σ'').
-Qed.
-
-Lemma isEtaExp_app_extends Σ Σ' ind k n :
-  extends Σ Σ' ->
-  wf_glob Σ' -> 
-  isEtaExp_app Σ ind k n ->
-  isEtaExp_app Σ' ind k n.
-Proof.
-  rewrite /isEtaExp_app.
-  rewrite /lookup_constructor_pars_args /lookup_inductive /lookup_minductive.
-  move=> ext wf.
-  destruct (lookup_env Σ _) eqn:hl => //.
-  rewrite (extends_lookup wf ext hl) /= //.
-Qed.
-
-Lemma isEtaExp_extends Σ Σ' t : 
-  extends Σ Σ' ->
-  wf_glob Σ' ->
-  isEtaExp Σ t ->
-  isEtaExp Σ' t.
-Proof.
-  intros ext wf.
-  funelim (isEtaExp Σ t); simp_eta => //; rtoProp; intuition eauto; rtoProp; intuition auto.
-  - eapply In_All in H; solve_all.
-  - eapply isEtaExp_app_extends; tea.
-  - eapply In_All in H0. solve_all.
-  - eapply In_All in H; solve_all.
-  - eapply In_All in H; solve_all.
-  - eapply In_All in H; solve_all.
-    rewrite isEtaExp_Constructor //. rtoProp; intuition auto.
-    eapply isEtaExp_app_extends; tea.
-    solve_all.
-  - eapply In_All in H0. apply isEtaExp_mkApps_intro; eauto. solve_all.
-Qed.
-
-
-Lemma isEtaExp_extends_decl Σ Σ' t : 
-  extends Σ Σ' ->
-  wf_glob Σ' ->
-  isEtaExp_decl Σ t ->
-  isEtaExp_decl Σ' t.
-Proof.
-  intros ext wf; destruct t; cbn => //.
-  rewrite /isEtaExp_constant_decl; destruct (cst_body c) => /= //.
-  now eapply isEtaExp_extends.
-Qed.
-
-Lemma isEtaExp_lookup {Σ kn d}: 
-  isEtaExp_env Σ -> wf_glob Σ ->
-  lookup_env Σ kn = Some d ->
-  isEtaExp_decl Σ d.
-Proof.
-  move=> etaΣ wfΣ.
-  move/(isEtaExp_lookup_ext etaΣ) => [Σ' []] ext hd.
-  now eapply isEtaExp_extends_decl.
-Qed.
-
 Arguments lookup_inductive_pars_constructor_pars_args {Σ ind n pars args}.
 
 Lemma strip_tApp {Σ : GlobalContextMap.t} f a : isEtaExp Σ f -> isEtaExp Σ a -> strip Σ (EAst.tApp f a) = EAst.tApp (strip Σ f) (strip Σ a).
@@ -629,7 +460,7 @@ Proof.
   move=> etaf etaa.
   pose proof (isEtaExp_mkApps_intro _ _ [a] etaf).
   forward H by eauto.
-  move/isEtaExp_tApp': H.
+  move/isEtaExp_mkApps: H.
   destruct decompose_app eqn:da.
   destruct construct_viewc eqn:cv => //.
   { intros [? [? []]]. rewrite H0 /=.
@@ -644,7 +475,7 @@ Proof.
     assert (pars - #|remove_last l| = 0) as ->.
     2:{ rewrite skipn_0 //. }
     rewrite H0 in etaf.
-    rewrite isEtaExp_mkApps // in etaf.
+    rewrite isEtaExp_mkApps_napp // in etaf.
     simp construct_viewc in etaf.
     move/andP: etaf => []. rewrite /isEtaExp_app hl.
     move/Nat.leb_le. lia. }
@@ -773,310 +604,6 @@ Module Fast.
 
 End Fast.
 
-Scheme eval_nondep := Minimality for Ee.eval Sort Prop.
-
-Fixpoint eval_depth {wfl : Ee.WcbvFlags} {Σ : EAst.global_declarations} {t1 t2 : EAst.term} (ev : Ee.eval Σ t1 t2) { struct ev } : nat.
-Proof.
-  rename eval_depth into aux.
-  destruct ev.
-  all:try match goal with
-  | [ H : Ee.eval _ _ _, H' : Ee.eval _ _ _, H'' : Ee.eval _ _ _ |- _ ] => 
-    apply aux in H; apply aux in H'; apply aux in H''; exact (S (Nat.max H (Nat.max H' H'')))
-  | [ H : Ee.eval _ _ _, H' : Ee.eval _ _ _ |- _ ] => 
-    apply aux in H; apply aux in H'; exact (S (Nat.max H H'))
-  | [ H : Ee.eval _ _ _ |- _ ] => apply aux in H; exact (S H)
-  end.
-  exact 1.
-Defined.
-
-Lemma eval_construct_size  {fl : Ee.WcbvFlags} [Σ kn c args e] : 
-  forall (ev : Ee.eval Σ (mkApps (tConstruct kn c) args) e),
-  ∑ args', (e = mkApps (tConstruct kn c) args') ×
-  All2 (fun x y => ∑ ev' : Ee.eval Σ x y, eval_depth ev' < eval_depth ev) args args'.
-Proof.
-  revert e; induction args using rev_ind; intros e.
-  - intros ev. depelim ev. exists []=> //.
-  - intros ev. revert ev.
-    rewrite mkApps_app /=.
-    intros ev.
-    depelim ev; try solve_discr.
-    destruct (IHargs _ ev1) as [? []]. solve_discr.
-    all:try specialize (IHargs _ ev1) as [? []]; try solve_discr.
-    * subst f'. 
-      exists (x0 ++ [a'])%list.
-      rewrite mkApps_app /= //.
-      cbn in i. split => //. eapply All2_app; eauto.
-      eapply All2_impl; tea. cbn. intros ? ? [ev' ?]. exists ev'. lia.
-      constructor. exists ev2. lia. constructor.
-    * now cbn in i.
-Qed.
-
-Lemma eval_mkApps_rect :
-∀ (wfl : Ee.WcbvFlags) (Σ : EAst.global_declarations) 
-  (P : EAst.term → EAst.term → Type),
-  (∀ a t t' : EAst.term,
-	 Ee.eval Σ a EAst.tBox
-     → P a EAst.tBox → Ee.eval Σ t t' → P t t' → P (EAst.tApp a t) EAst.tBox)
-  → (∀ (f0 : EAst.term) (na : name) (b a a' res : EAst.term),
-       Ee.eval Σ f0 (EAst.tLambda na b)
-       → P f0 (EAst.tLambda na b)
-         → Ee.eval Σ a a'
-           → P a a'
-             → Ee.eval Σ (ECSubst.csubst a' 0 b) res
-               → P (ECSubst.csubst a' 0 b) res → P (EAst.tApp f0 a) res)
-    → (∀ (na : name) (b0 b0' b1 res : EAst.term),
-         Ee.eval Σ b0 b0'
-         → P b0 b0'
-           → Ee.eval Σ (ECSubst.csubst b0' 0 b1) res
-             → P (ECSubst.csubst b0' 0 b1) res → P (EAst.tLetIn na b0 b1) res)
-      → (∀ (ind : inductive) (pars : nat) (discr : EAst.term) 
-           (c : nat) (args : list EAst.term) (brs : 
-                                              list 
-                                                (list name × EAst.term)) 
-           (br : list name × EAst.term) (res : EAst.term),
-           Ee.eval Σ discr (EAst.mkApps (EAst.tConstruct ind c) args)
-           → P discr (EAst.mkApps (EAst.tConstruct ind c) args)
-             → inductive_isprop_and_pars Σ ind = Some (false, pars)
-               → nth_error brs c = Some br
-                 → #|skipn pars args| = #|br.1|
-                   → Ee.eval Σ (iota_red pars args br) res
-                     → P (iota_red pars args br) res
-                       → P (EAst.tCase (ind, pars) discr brs) res)
-        → (∀ (ind : inductive) (pars : nat) (discr : EAst.term) 
-             (brs : list (list name × EAst.term)) 
-             (n : list name) (f3 res : EAst.term),
-             Ee.with_prop_case
-             → Ee.eval Σ discr EAst.tBox
-               → P discr EAst.tBox
-                 → inductive_isprop_and_pars Σ ind = Some (true, pars)
-                   → brs = [(n, f3)]
-                     → Ee.eval Σ (ECSubst.substl (repeat EAst.tBox #|n|) f3)
-                         res
-                       → P (ECSubst.substl (repeat EAst.tBox #|n|) f3) res
-                         → P (EAst.tCase (ind, pars) discr brs) res)
-          → (∀ (f4 : EAst.term) (mfix : EAst.mfixpoint EAst.term) 
-               (idx : nat) (argsv : list EAst.term) 
-               (a av fn res : EAst.term),
-               Ee.eval Σ f4 (EAst.mkApps (EAst.tFix mfix idx) argsv)
-               → P f4 (EAst.mkApps (EAst.tFix mfix idx) argsv)
-                 → Ee.eval Σ a av
-                   → P a av
-                     → Ee.cunfold_fix mfix idx = Some (#|argsv|, fn)
-                       → Ee.eval Σ (EAst.tApp (EAst.mkApps fn argsv) av) res
-                         → P (EAst.tApp (EAst.mkApps fn argsv) av) res
-                           → P (EAst.tApp f4 a) res)
-            → (∀ (f5 : EAst.term) (mfix : EAst.mfixpoint EAst.term) 
-                 (idx : nat) (argsv : list EAst.term) 
-                 (a av : EAst.term) (narg : nat) (fn : EAst.term),
-                 Ee.eval Σ f5 (EAst.mkApps (EAst.tFix mfix idx) argsv)
-                 → P f5 (EAst.mkApps (EAst.tFix mfix idx) argsv)
-                   → Ee.eval Σ a av
-                     → P a av
-                       → Ee.cunfold_fix mfix idx = Some (narg, fn)
-                         → #|argsv| < narg
-                           → P (EAst.tApp f5 a)
-                               (EAst.tApp
-                                  (EAst.mkApps (EAst.tFix mfix idx) argsv) av))
-              → (∀ (ip : inductive × nat) (mfix : EAst.mfixpoint EAst.term) 
-                   (idx : nat) (args : list EAst.term) 
-                   (narg : nat) discr (fn : EAst.term) (brs : 
-                                                 list 
-                                                 (list name × EAst.term)) 
-                   (res : EAst.term),
-                   Ee.cunfold_cofix mfix idx = Some (narg, fn)
-                   -> Ee.eval Σ discr (EAst.mkApps (EAst.tCoFix mfix idx) args)
-                   -> P discr (EAst.mkApps (EAst.tCoFix mfix idx) args)
-                   → Ee.eval Σ (EAst.tCase ip (EAst.mkApps fn args) brs) res
-                     → P (EAst.tCase ip (EAst.mkApps fn args) brs) res
-                       → P
-                           (EAst.tCase ip discr brs)
-                           res)
-                → (∀ (p : projection) (mfix : EAst.mfixpoint EAst.term) 
-                     (idx : nat) (args : list EAst.term) 
-                     (narg : nat) discr (fn res : EAst.term),
-                     Ee.cunfold_cofix mfix idx = Some (narg, fn)
-                     -> Ee.eval Σ discr (EAst.mkApps (EAst.tCoFix mfix idx) args)
-                     -> P discr (EAst.mkApps (EAst.tCoFix mfix idx) args)
-                     → Ee.eval Σ (EAst.tProj p (EAst.mkApps fn args)) res
-                       → P (EAst.tProj p (EAst.mkApps fn args)) res
-                         → P
-                             (EAst.tProj p discr) res)
-                  → (∀ (c : kername) (decl : EAst.constant_body) 
-                       (body : EAst.term),
-                       declared_constant Σ c decl
-                       → ∀ res : EAst.term,
-                           EAst.cst_body decl = Some body
-                           → Ee.eval Σ body res
-                             → P body res → P (EAst.tConst c) res)
-                    → (∀ (i : inductive) (pars arg : nat) 
-                         (discr : EAst.term) (args : list EAst.term) 
-                         (res : EAst.term),
-                         Ee.eval Σ discr
-                           (EAst.mkApps (EAst.tConstruct i 0) args)
-                         → P discr (EAst.mkApps (EAst.tConstruct i 0) args)
-                           → inductive_isprop_and_pars Σ i = Some (false, pars)
-                             → Ee.eval Σ (nth (pars + arg) args tDummy) res
-                               → P (nth (pars + arg) args tDummy) res
-                                 → P (EAst.tProj (i, pars, arg) discr) res)
-                      → (∀ (i : inductive) (pars arg : nat) 
-                           (discr : EAst.term),
-                           Ee.with_prop_case
-                           → Ee.eval Σ discr EAst.tBox
-                             → P discr EAst.tBox
-                               → inductive_isprop_and_pars Σ i = Some (true, pars)
-                                 → P (EAst.tProj (i, pars, arg) discr)
-                                     EAst.tBox)
-                        → (∀ (f11 f' : EAst.term) a a' ,
-                             forall (ev : Ee.eval Σ f11 f'),
-                              P f11 f' ->
-                              (forall t u (ev' : Ee.eval Σ t u), eval_depth ev' <= eval_depth ev -> P t u)
-                            → ~~
-                                 (EAst.isLambda f' || Ee.isFixApp f'
-                                  || isBox f')
-                                 → Ee.eval Σ a a'
-                                → P a a'
-                          →  P (EAst.tApp f11 a) (EAst.tApp f' a'))
-                                  
-                          → (∀ t : EAst.term, Ee.atom t → P t t)
-                            → ∀ t t0 : EAst.term, Ee.eval Σ t t0 → P t t0.
-Proof.
-  intros.
-  pose proof (p := @Fix_F { t : _ & { t0 : _ & Ee.eval Σ t t0 }}).
-  specialize (p (MR lt (fun x => eval_depth x.π2.π2))).
-  set(foo := existT _ t (existT _ t0 H) :  { t : _ & { t0 : _ & Ee.eval Σ t t0 }}).
-  change t with (projT1 foo).
-  change t0 with (projT1 (projT2 foo)).
-  change H with (projT2 (projT2 foo)).
-  revert foo.
-  match goal with
-    |- let foo := _ in @?P foo => specialize (p (fun x => P x))
-  end.
-  forward p.
-  2:{ apply p. apply measure_wf, lt_wf. }
-  clear p.
-  clear t t0 H.
-  intros (t & t0 & ev). 
-  intros IH.
-  set (IH' t t0 H := IH (t; t0; H)). clearbody IH'; clear IH; rename IH' into IH.
-  cbn in IH. unfold MR in IH; cbn in IH. cbn.
-  destruct ev.
-  all:try solve [match goal with
-  | [ H : _ |- _ ] =>
-    eapply H; tea; unshelve eapply IH; tea; cbn; lia
-  end].
-  cbn in IH.
-  eapply X11; tea; eauto; try unshelve eapply IH; tea; cbn; try lia.
-  Unshelve. 2:exact ev1. intros. unshelve eapply IH; tea. cbn. lia.
-Qed.
-
-Lemma eval_etaexp {fl : Ee.WcbvFlags} {Σ a a'} : 
-  isEtaExp_env Σ ->
-  wf_glob Σ ->
-  Ee.eval Σ a a' -> isEtaExp Σ a -> isEtaExp Σ a'.
-Proof.
-  intros etaΣ wfΣ.
-  induction 1 using eval_mkApps_rect.
-  all:try simp isEtaExp; rewrite -!isEtaExp_equation_1 => //.
-  - move/isEtaExp_tApp'.
-    destruct decompose_app eqn:da.
-    destruct construct_viewc eqn:vc.
-    * move => [hl [hf [ha /andP[] ise etal]]].
-      rewrite hf in H. eapply eval_construct in H as [? []]; solve_discr.
-    * move/and4P => [] etat etal etaf etaa.
-      eapply IHeval3; eauto. 
-      move: (IHeval1 etaf); simp_eta => etab.
-      eapply etaExp_csubst; eauto.
-  - rtoProp; intuition eauto using etaExp_csubst.
-  - rtoProp; intuition eauto using isEtaExp_substl.
-    eapply IHeval2. rewrite /iota_red.
-    eapply isEtaExp_substl; eauto. solve_all.
-    destruct args => //. rewrite skipn_nil. constructor.
-    rewrite isEtaExp_Constructor // in H4.
-    eapply All_skipn. move/andP: H4 => []. repeat solve_all.
-    eapply forallb_nth_error in H6; tea.
-    now erewrite H1 in H6.
-  - rtoProp; intuition auto.
-    eapply IHeval2. eapply isEtaExp_substl.
-    now apply forallb_repeat.
-    rewrite H2 in H6. simpl in H6.
-    now move/andP: H6.
-  - intros ise.
-    eapply IHeval3.
-    apply isEtaExp_tApp' in ise.
-    destruct decompose_app eqn:da.
-    destruct (construct_viewc t) eqn:cv.
-    * destruct ise as [? [? []]]. rewrite H4 in H.
-      eapply eval_construct in H as [? []];solve_discr.
-    * move/and4P: ise => [] iset isel isef isea.
-      rewrite -[EAst.tApp _ _](mkApps_app _ _ [av]).
-      specialize (IHeval1 isef).
-      rewrite isEtaExp_mkApps // in IHeval1.
-      simp construct_viewc in IHeval1.
-      move/andP: IHeval1 => [] evfix evargs.
-      eapply isEtaExp_mkApps_intro.
-      eapply isEtaExp_cunfold_fix; tea.
-      simp isEtaExp in evfix.
-      eapply All_app_inv. now solve_all. constructor; auto.
-  - intros ise.
-    apply isEtaExp_tApp' in ise.
-    destruct decompose_app eqn:da.
-    destruct (construct_viewc t) eqn:cv.
-    * destruct ise as [? [? []]]. rewrite H4 in H.
-      eapply eval_construct in H as [? []]; solve_discr.
-    * move/and4P: ise => [] iset isel isef isea.
-      rewrite -[EAst.tApp _ _](mkApps_app _ _ [av]).
-      specialize (IHeval1 isef).
-      rewrite isEtaExp_mkApps // in IHeval1.
-      simp construct_viewc in IHeval1.
-      move/andP: IHeval1 => [] evfix evargs.
-      eapply isEtaExp_mkApps_intro => //.
-      eapply All_app_inv. now solve_all. constructor; auto.
-  - move=> /andP[] hdiscr hbrs. specialize (IHeval1 hdiscr).
-    move: IHeval1. rewrite isEtaExp_mkApps // /= => /andP[] hcof hargs.
-    eapply IHeval2. simp_eta. rtoProp; intuition auto.
-    apply isEtaExp_mkApps_intro; solve_all.
-    eapply (isEtaExp_cunfold_cofix _ mfix idx); tea.
-    simp_eta in hcof.
-  -  move=> hdiscr. specialize (IHeval1 hdiscr).
-    move: IHeval1. rewrite isEtaExp_mkApps // /= => /andP[] hcof hargs.
-    eapply IHeval2. simp_eta.
-    apply isEtaExp_mkApps_intro; solve_all.
-    eapply (isEtaExp_cunfold_cofix _ mfix idx); tea.
-    simp_eta in hcof.
-  - move=> _. eapply IHeval. eapply isEtaExp_lookup in H; tea.
-    now move: H; rewrite /isEtaExp_decl /= /isEtaExp_constant_decl H0 /=.
-  - intros hd.
-    eapply IHeval2. specialize (IHeval1 hd).
-    move: IHeval1.
-    rewrite nth_nth_error in H1 *.
-    destruct nth_error eqn:hnth.
-    rewrite isEtaExp_Constructor.
-    destruct args => //. now rewrite nth_error_nil in hnth.
-    move=> /andP[] _ hargs. eapply nth_error_forallb in hnth; tea.
-    depelim H0. now cbn in H1.
-  - move/isEtaExp_tApp'.
-    destruct decompose_app eqn:da.
-    destruct construct_viewc.
-    * move=> [] hl [] hf [] ha /andP[] hl' etal.
-      move: H H0. rewrite hf => H H0.
-      destruct (eval_construct_size H) as [args' []]. subst f'.
-      rewrite -[EAst.tApp _ _](mkApps_app _ _ [a']).
-      rewrite isEtaExp_Constructor.
-      apply/andP; split => //.
-      + len. eapply All2_length in a0. rewrite -a0.
-        rewrite (remove_last_last l a) // in hl'. len in hl'.
-        now cbn in hl'.
-      + solve_all.
-        rewrite (remove_last_last l a) // in etal.
-        eapply All_app in etal as [etal etaa].
-        depelim etaa. clear etaa. rewrite -ha in i.
-        eapply All_app_inv; try constructor; eauto.
-        clear -H0 a0 etal. solve_all.
-        destruct b as [ev Hev]. eapply (H0 _ _ ev) => //. lia.
-    * move/and4P => [] etat etal etaf etaa.
-      eapply (isEtaExp_mkApps_intro _ f' [a']); eauto.
-Qed.
-
 Lemma isLambda_mkApps' f l :
   l <> nil ->
   ~~ EAst.isLambda (EAst.mkApps f l).
@@ -1196,7 +723,7 @@ Lemma strip_mkApps_etaexp {Σ : GlobalContextMap.t} fn args :
 Proof.
   destruct (decompose_app fn) eqn:da.
   rewrite (decompose_app_inv da).
-  rewrite isEtaExp_mkApps. now eapply decompose_app_notApp.
+  rewrite isEtaExp_mkApps_napp. now eapply decompose_app_notApp.
   destruct construct_viewc eqn:vc.
   + move=> /andP[] hl0 etal0.
     rewrite -mkApps_app.
@@ -1214,6 +741,37 @@ Proof.
     rewrite vc. rewrite -mkApps_app !map_app //. 
 Qed.
 
+#[export] Instance Qpreserves_closedn Σ : closed_env Σ ->
+  Qpreserves (fun n x => closedn n x) Σ.
+Proof.
+  intros clΣ.
+  split.
+  - red. move=> n t.
+    destruct t; cbn; intuition auto; try solve [constructor; auto].
+    eapply on_evar; solve_all.
+    eapply on_letin; rtoProp; intuition auto.
+    eapply on_app; rtoProp; intuition auto.
+    eapply on_case; rtoProp; intuition auto. solve_all.
+    eapply on_fix. solve_all.
+    eapply on_cofix; solve_all.
+  - red. intros kn decl.
+    move/(lookup_env_closed clΣ).
+    unfold closed_decl. destruct EAst.cst_body => //.
+  - red. move=> n t args. rewrite closedn_mkApps. 
+    split; intros; rtoProp; intuition auto; solve_all.
+  - red. move=> n ci discr brs. simpl.
+    split; intros; rtoProp; intuition auto; solve_all.
+  - red. move=> n p discr. simpl.
+    split; intros; rtoProp; intuition auto; solve_all.
+  - red. move=> t args clt cll.
+    eapply closed_substl. solve_all. now rewrite Nat.add_0_r.
+  - red. move=> n mfix idx. cbn.
+    split; intros; rtoProp; intuition auto; solve_all.
+  - red. move=> n mfix idx. cbn.
+    split; intros; rtoProp; intuition auto; solve_all.
+  - red. now cbn.
+Qed.
+
 Lemma strip_eval {wfl:Ee.WcbvFlags} {Σ : GlobalContextMap.t} t v :
   closed_env Σ ->
   isEtaExp_env Σ ->
@@ -1223,287 +781,147 @@ Lemma strip_eval {wfl:Ee.WcbvFlags} {Σ : GlobalContextMap.t} t v :
   isEtaExp Σ t ->
   Ee.eval (strip_env Σ) (strip Σ t) (strip Σ v).
 Proof.
-  intros clΣ etaΣ wfΣ ev.
-  induction ev using eval_mkApps_rect; simpl in *. try solve [econstructor; eauto].
-
-  - move/andP => [] cla clt.
-    move/isEtaExp_tApp'.
-    destruct decompose_app as [hd args] eqn:da.
-    destruct (construct_viewc hd) eqn:cv.
-    * move=> [] argsn [] ha [] ht /andP[] etaind etaargs.
-      rewrite ha in ev1. elimtype False.
-      eapply eval_construct in ev1 as [ex []]. solve_discr.
-    * move=> /and4P [] etat0 etaargs etaa etat.
-      rewrite strip_tApp //.
-      econstructor; eauto.
-
-  - move/andP => [] clf cla.
-    move/isEtaExp_tApp'.
-    destruct decompose_app as [hd args] eqn:da.
-    destruct (construct_viewc hd) eqn:cv.
-    * intros [? [? []]].
-      rewrite H0 in ev1. elimtype False; eapply eval_construct in ev1 as [? []]. solve_discr.
-    * move=> /and4P[] etat etaargs etaf etaa.
-      specialize (IHev1 clf etaf).
-      specialize (IHev2 cla etaa).
-      rewrite strip_tApp //.
-      eapply eval_etaexp in etaf; tea.
-      eapply eval_etaexp in etaa; tea. simp_eta in etaf.
-      eapply eval_closed in ev2; tea.
-      eapply eval_closed in ev1; tea.
-      econstructor; eauto. now simp_strip in IHev1.
-      rewrite strip_csubst // in IHev3.
-      apply IHev3. eapply closed_csubst => //.
-      eapply etaExp_csubst; eauto.
-
-  - move/andP => [] clb0 clb1.
-    simp_eta. move/andP => [] etb0 etb1.
-    specialize (IHev1 clb0 etb0).
-    eapply eval_closed in clb0; tea; eauto.
-    simp_strip.
-    eapply eval_etaexp in etb0; tea.
-    forward IHev2.
-    eapply closed_csubst => //.
-    forward IHev2.
-    now eapply etaExp_csubst.
-    rewrite strip_csubst // in IHev2.
+  intros clΣ etaΣ wfΣ ev clt etat.
+  revert t v clt etat ev.
+  apply (eval_preserve_mkApps_ind wfl Σ (fun x y => Ee.eval (strip_env Σ) (strip Σ x) (strip Σ y))
+    (fun n x => closedn n x) (Qpres := Qpreserves_closedn Σ clΣ)) => //.
+  { intros. eapply eval_closed; tea. }
+  all:intros; simpl in *; try solve [econstructor; eauto].
+  all:repeat destruct_nary_times.
+  - rewrite strip_tApp //.
     econstructor; eauto.
 
-  - move/andP => [] cld clbrs. rewrite strip_mkApps // in IHev1.
-    have := (eval_closed _ clΣ _ _ cld ev1); rewrite closedn_mkApps => /andP[] _ clargs.
-    simp_eta; move=> /andP[] etad etabrs.
-    specialize (IHev1 cld etad).
-    cbn [construct_viewc] in IHev1.
-    move: (is_propositional_strip Σ ind). rewrite H.
-    intros isps.
-    destruct lookup_inductive_pars as [pars'|] eqn:hlook.
-    simp_strip. set (brs' := map _ brs). cbn -[strip].
-    assert (pars' = pars).
-    { clear -H hlook.
-      apply lookup_inductive_pars_is_prop_and_pars in H.
-      congruence. }
-    subst pars'.
-    econstructor; tea.
-    * rewrite nth_error_map H0 //.
-    * len. now rewrite -H1.
-    * have etaargs : forallb (isEtaExp Σ) args.
-      { eapply eval_etaexp in ev1; tea.
-        rewrite isEtaExp_Constructor in ev1.
-        now move/andP: ev1 => []. }
-      have etabr : isEtaExp Σ br.2.
-      { now eapply nth_error_forallb in etabrs; tea. }
-      rewrite strip_iota_red // in IHev2.
-      eapply eval_closed in ev1 => //.
-      rewrite /iota_red. rewrite skipn_0.
-      eapply IHev2.
-      eapply closed_iota_red => //; tea.
-      eapply nth_error_forallb in clbrs; tea. cbn in clbrs.
-      now rewrite Nat.add_0_r in clbrs.
-      now eapply isEtaExp_iota_red.
-    * eapply lookup_inductive_pars_is_prop_and_pars in H. congruence.
+  - rewrite strip_tApp //. simp_strip in e1.
+    econstructor; eauto. 
+    rewrite strip_csubst // in e. now simp_eta in i10.
+
+  - simp_strip. 
+    rewrite strip_csubst // in e.
+    econstructor; eauto.
+
+  - simp_strip.
+    set (brs' := map _ brs). cbn -[strip].
+    cbn in H3.
+    rewrite strip_mkApps // /= in e0.
+    apply lookup_inductive_pars_is_prop_and_pars in H2 as H1'.
+    rewrite H1' in e0.
+    pose proof (is_propositional_strip Σ ind). rewrite H2 in H1.
+    econstructor; eauto.
+    * rewrite nth_error_map H3 //.
+    * now len.
+    * cbn -[strip].
+      have etaargs : forallb (isEtaExp Σ) args.
+      { rewrite isEtaExp_Constructor in i6.
+        now move/andP: i6 => []. }
+      rewrite strip_iota_red // in e.
+      rewrite closedn_mkApps in i4. now move/andP: i4.
+      cbn. now eapply nth_error_forallb in H; tea.
   
-  - move/andP => [] cld clbrs. simp_eta.
-    move/andP => [] etad etabrs.
-    subst brs. cbn in clbrs. rewrite Nat.add_0_r andb_true_r in clbrs.
-    cbn in etabrs; rewrite andb_true_r in etabrs.
-    rewrite strip_substl // in IHev2. 
+  - subst brs. cbn in H4.
+    rewrite andb_true_r in H4.
+    rewrite strip_substl // in e.
     eapply All_forallb, All_repeat => //.
     eapply All_forallb, All_repeat => //.
-    rewrite map_strip_repeat_box in IHev2.
+    rewrite map_strip_repeat_box in e.
     simp_strip. set (brs' := map _ _).
     cbn -[strip]. eapply Ee.eval_iota_sing => //.
-    apply IHev1 => //.
-    now move: (is_propositional_strip Σ ind); rewrite H0.
-    eapply IHev2.
-    eapply closed_substl.
-    eapply All_forallb, All_repeat => //.
-    now rewrite repeat_length Nat.add_0_r.
-    eapply isEtaExp_substl => //.
-    apply forallb_repeat => //.
+    now move: (is_propositional_strip Σ ind); rewrite H2.
 
-  - move/andP => [] clf cla. rewrite strip_mkApps // in IHev1.
-    move/isEtaExp_tApp'. simpl in IHev1.
-    destruct decompose_app eqn:da.
-    destruct (construct_viewc t) eqn:vc.
-    { move=> [] hl [] hf [] ha /andP[] etaind etal.
-      rewrite hf in ev1.
-      eapply eval_construct in ev1 as [? []]. solve_discr. }
-    move=> /and4P[] etat etal etaf etaa.
-    rewrite strip_tApp //.
-    move: (eval_closed _ clΣ _ _ clf ev1); tea.
-    rewrite closedn_mkApps.
-    move/andP => [] clfix clargs.
-    move: (eval_etaexp etaΣ wfΣ ev1 etaf).
-    rewrite isEtaExp_mkApps // /= => /andP[] etafix etaargs.
-    specialize (IHev2 cla etaa).
-    simp_strip in IHev1.
-    eapply Ee.eval_fix.
-    * eapply IHev1 => //.
-    * eapply IHev2.
+  - rewrite strip_tApp //.
+    rewrite strip_mkApps // /= in e1.
+    simp_strip in e1.
+    eapply Ee.eval_fix; tea.
     * rewrite map_length.
       eapply strip_cunfold_fix; tea.
       eapply closed_fix_subst. tea.
-      simp_eta in etafix.
-    * forward IHev3.
-      { apply /andP; split. rewrite closedn_mkApps. apply /andP; split => //.
-        eapply closed_cunfold_fix; tea. eapply eval_closed in ev2; tea. }
-      assert (etafn : isEtaExp Σ fn).
-      { eapply isEtaExp_cunfold_fix => //; tea. simp_eta in etafix. }
-      forward_keep IHev3.
-      { rewrite -[tApp _ _](mkApps_app _ _ [av]). apply isEtaExp_mkApps_intro => //.
-        eapply All_app_inv; try econstructor; eauto. solve_all. eapply eval_etaexp; tea. }
-      move: H0 IHev3. clear IHev1.
+      move: i8; rewrite closedn_mkApps => /andP[] //.
+      move: i10; rewrite isEtaExp_mkApps_napp // /= => /andP[] //. simp_eta.
+    * move: e.
       rewrite -[tApp _ _](mkApps_app _ _ [av]).
-      rewrite -[tApp _ _](mkApps_app _ _ [strip _ av]). move=> _.
+      rewrite -[tApp _ _](mkApps_app _ _ [strip _ av]).
       rewrite strip_mkApps_etaexp // map_app //.
 
-  - move/andP => [] clf cla.
-    move/isEtaExp_tApp'.
-    destruct decompose_app eqn:da.
-    destruct (construct_viewc t).
-    { move=> [] hl [] hf [] ha /andP[] etaind etal.
-      rewrite hf.
-      rewrite hf in ev1. eapply eval_construct in ev1 as [? []]; solve_discr. }
-    move=> /and4P[] etat etal etaf5 etaa.
+  - rewrite strip_tApp //.
     rewrite strip_tApp //.
-    rewrite strip_tApp. eapply eval_etaexp; eauto. eapply eval_etaexp; eauto.
     rewrite strip_mkApps //. simpl.
     simp_strip. set (mfix' := map _ _). simpl.
-    do 2 forward IHev1 by auto.
-    do 2 forward IHev2 by auto.
-    rewrite strip_mkApps // in IHev1. simpl in IHev1.
+    rewrite strip_mkApps // /= in e0. simp_strip in e0.
     eapply Ee.eval_fix_value; tea.
-    simp_strip in IHev1. eapply IHev1.
     eapply strip_cunfold_fix; eauto.
     eapply closed_fix_subst => //.
-    { eapply eval_closed in ev1; tea.
-      rewrite closedn_mkApps in ev1. now move/andP: ev1. }
-    { eapply eval_etaexp in ev1; tea.
-      rewrite isEtaExp_mkApps // in ev1. simpl in ev1.
-      move/andP: ev1 => []. now simp isEtaExp. }
+    { move: i4.
+      rewrite closedn_mkApps. now move/andP => []. }
+    { move: i6. rewrite isEtaExp_mkApps_napp // /= => /andP[] //. now simp isEtaExp. }
     now rewrite map_length. 
 
-  - move => /andP[] cld clbrs.
-    specialize (IHev1 cld).
-    simp_eta. move=> /andP[] etad etabrs.
-    forward IHev1 by auto.
-    move: (eval_etaexp etaΣ wfΣ ev1 etad).
-    rewrite isEtaExp_mkApps /= //. move/andP => [] etafix etaargs.
-    move: (eval_closed _ clΣ _ _ cld ev1).
-    rewrite closedn_mkApps. move=> /andP [] clfix clargs.
-    forward IHev2.
-    { rewrite clbrs andb_true_r. rewrite closedn_mkApps clargs andb_true_r.
-      eapply closed_cunfold_cofix; tea. }
-    forward IHev2.
-    { simp_eta. rewrite etabrs andb_true_r.
-      eapply isEtaExp_mkApps_intro.
-      eapply isEtaExp_cunfold_cofix; tea. simp_eta in etafix. solve_all. }
-    rewrite strip_mkApps // /= in IHev1. simp_strip in IHev1.
-    simp_strip in IHev2.
-    simp_strip. set (brs' := map _ _) in *; simpl.
-    simp_eta in etafix.
+  - rewrite strip_tApp //. simp_strip in e0.
+    simp_strip in e1.
+    eapply Ee.eval_fix'; tea.
+    eapply strip_cunfold_fix; tea.
+    { eapply closed_fix_subst => //. }
+    { simp isEtaExp in i10. }
+    rewrite strip_tApp // in e.
+
+  - simp_strip.
+    rewrite strip_mkApps // /= in e0.
+    simp_strip in e.
+    simp_strip in e0.
+    set (brs' := map _ _) in *; simpl.
     eapply Ee.eval_cofix_case; tea.
     eapply strip_cunfold_cofix; tea => //.
-    { eapply closed_cofix_subst; tea. }
-    rewrite strip_mkApps_etaexp in IHev2.
-    { eapply isEtaExp_cunfold_cofix; tea. }
-    exact IHev2.
+    { eapply closed_cofix_subst; tea.
+      move: i5; rewrite closedn_mkApps => /andP[] //. }
+    { move: i7. rewrite isEtaExp_mkApps_napp // /= => /andP[] //. now simp isEtaExp. }
+    rewrite strip_mkApps_etaexp // in e.
 
-  - move=> cld. simp_eta => etad.
-    specialize (IHev1 cld).
-    simp_eta.
-    forward IHev1 by auto.
-    move: (eval_etaexp etaΣ wfΣ ev1 etad).
-    rewrite isEtaExp_mkApps /= //. move/andP => [] etafix etaargs.
-    move: (eval_closed _ clΣ _ _ cld ev1).
-    rewrite closedn_mkApps. move=> /andP [] clfix clargs.
-    forward IHev2.
-    { rewrite closedn_mkApps clargs andb_true_r.
-      eapply closed_cunfold_cofix; tea. }
-    forward IHev2.
-    { simp_eta. 
-      eapply isEtaExp_mkApps_intro.
-      eapply isEtaExp_cunfold_cofix; tea. simp_eta in etafix. solve_all. }
-    destruct p as [[ind pars] arg].
-    simp_strip. simp_eta in etafix.
-    simp_strip in IHev1. simp_strip in IHev2.
-    rewrite strip_mkApps // /= in IHev1 IHev2.
-    simp_strip in IHev1. 
-    rewrite strip_mkApps_etaexp in IHev2.
-    now eapply isEtaExp_cunfold_cofix; tea.
+  - destruct p as [[ind pars] arg].
+    simp_strip. 
+    simp_strip in e.
+    rewrite strip_mkApps // /= in e0.
+    simp_strip in e0.
+    rewrite strip_mkApps_etaexp // in e.
+    simp_strip in e0.
     eapply Ee.eval_cofix_proj; tea.
     eapply strip_cunfold_cofix; tea.
-    { eapply closed_cofix_subst; tea. }
+    { eapply closed_cofix_subst; tea.
+      move: i4; rewrite closedn_mkApps => /andP[] //. }
+    { move: i6. rewrite isEtaExp_mkApps_napp // /= => /andP[] //. now simp isEtaExp. }
   
   - econstructor. red in H |- *.
     rewrite lookup_env_strip H //.
     now rewrite /strip_constant_decl H0.
-    apply IHev.
-    eapply lookup_env_closed in clΣ; tea.
-    move: clΣ. rewrite /closed_decl H0 //.
-    eapply isEtaExp_lookup in H; tea.
-    unfold isEtaExp_decl, isEtaExp_constant_decl in H.
-    now rewrite H0 in H.
+    exact e.
   
-  - move=> cld. simp_eta => etad.
-    move: (eval_closed _ clΣ _ _ cld ev1); rewrite closedn_mkApps /= => clargs.
-    move: (eval_etaexp etaΣ wfΣ ev1 etad); rewrite isEtaExp_mkApps // /= => /andP[] etaind etargs.
-    simp_strip.
-    rewrite strip_mkApps // /= in IHev1.
-    rewrite (lookup_inductive_pars_is_prop_and_pars _ _ _ _ H) in IHev1.
+  - simp_strip.
+    rewrite strip_mkApps // /= in e0.
+    rewrite (lookup_inductive_pars_is_prop_and_pars _ _ _ _ H1) in e0.
     eapply Ee.eval_proj; eauto.
-    move: (is_propositional_strip Σ i). now rewrite H. simpl.
-    rewrite nth_nth_error in ev2 IHev2 *. rewrite nth_nth_error.
+    move: (is_propositional_strip Σ i). now rewrite H1. simpl.
+    rewrite nth_nth_error in e. rewrite nth_nth_error.
     rewrite nth_error_skipn nth_error_map.
     destruct nth_error eqn:hnth => /= //.
-    * eapply IHev2.
-      eapply nth_error_forallb in hnth; tea.
-      eapply nth_error_forallb in hnth; tea.
-    * depelim ev2. depelim i0.
 
-  - move=> cld. simp_eta => etad.
-    specialize (IHev cld etad).
-    simp_strip. eapply Ee.eval_proj_prop => //.
-    move: (is_propositional_strip Σ i); now rewrite H0.
+  - simp_strip. eapply Ee.eval_proj_prop => //.
+    move: (is_propositional_strip Σ i); now rewrite H2.
 
-  - move/andP => [] clf cla'.
-    move/isEtaExp_tApp'.
-    destruct decompose_app eqn:da.
-    destruct construct_viewc eqn:cv.
-    intros [? [? []]].
-    rewrite (decompose_app_inv da).
-    rewrite strip_mkApps // cv.
-    move/andP: H4 => []. rewrite /isEtaExp_app.
-    destruct lookup_constructor_pars_args as [[pars args]|] eqn:dp => //.
-    rewrite (lookup_inductive_pars_constructor_pars_args dp).
-    move/Nat.leb_le => hl hf.
-    move: ev1 H. rewrite H2 => ev1 IH.
-    destruct (eval_construct_size ev1) as [args' [hf' hargs']].
-    rewrite hf'.
-    rewrite -[EAst.tApp _ _](mkApps_app _ _ [a']).
-    rewrite strip_mkApps // cv (lookup_inductive_pars_constructor_pars_args dp).
-    eapply eval_mkApps_Construct, All2_skipn.
-    rewrite {1}(remove_last_last l a) //.
-    rewrite !map_app.
-    assert (forallb (closedn 0) l).
-    { eapply decompose_app_inv in da.
-      assert (closed (tApp f11 a)) by (cbn; rtoProp; intuition).
-      rewrite da in H. now rewrite closedn_mkApps in H. }
-    * eapply forallb_All in hf.
-      eapply forallb_All in H.
-      rewrite [l](remove_last_last l a) // in hf H.
-      eapply All_app in hf as [hremove ha].
-      eapply All_app in H as [closedrem closeda].
-      apply All2_app; eauto.
-      2:{ constructor; eauto. rewrite -H3 //.
-        rewrite -H3 in ha; depelim ha.
-        eapply IHev2 => //. }
-      solve_all. destruct b as [evxy Hev]. eapply (IH _ _ evxy) => //. lia.
-    * move/and4P => [] etat etal etaf etaa.
-    rewrite !strip_tApp //. all:eauto using eval_etaexp.
-    constructor; eauto.
-    move: H0. eapply contraNN.
+  - rewrite strip_tApp //.
+    rewrite strip_tApp //.
+    eapply Ee.eval_app_cong; tea.
+    move: H2. eapply contraNN.
     rewrite -strip_isLambda -strip_isFixApp -strip_isBox //.
+    rewrite -strip_isFix //.
+  
+  - rewrite strip_mkApps // /=.
+    rewrite strip_mkApps // /=.
+    destruct (lookup_inductive_pars) eqn:hlook.
+    * eapply Ee.eval_mkApps_Construct.
+      eapply All2_skipn, All2_map.
+      eapply All2_impl; tea; cbn -[strip].
+      intros x y []; auto.
+    * eapply Ee.eval_mkApps_Construct.
+      eapply All2_map.
+      eapply All2_impl; tea; cbn -[strip].
+      intros x y []; auto.
   
   - destruct t => //.
     all:constructor; eauto.
@@ -1521,7 +939,7 @@ Proof.
   - destruct a as [kn' d]. intros. depelim H.
     cbn in H, H0.
     destruct d as []; simpl; destruct KernameSet.mem.
-    + cbn [ETyping.closed_env forallb]. cbn.
+    + cbn [EGlobalEnv.closed_env forallb]. cbn.
       constructor => //. eapply IHdecls => //.
     + eapply IHdecls => //.
     + constructor; auto.
@@ -1564,55 +982,3 @@ Lemma erase_global_wf_glob Σ deps :
   let Σ' := erase_global deps Σ in
   wf_glob Σ'.
 Proof. eapply erase_global_decls_wf_glob. Qed.
-
-(*
-Lemma strip_correct (wfl := Ee.default_wcbv_flags) (Σ : wf_env) univs wfext t v Σ' t' :
-  let Σext := make_wf_env_ext Σ univs wfext in
-  forall wt : welltyped Σext [] t,
-  erase Σext [] t wt = t' ->
-  erase_global (term_global_deps t') Σ = Σ' ->
-  isEtaExp_env Σ' ->
-  isEtaExp Σ' t' ->
-  PCUICWcbvEval.eval Σ t v ->
-  ∃ v' : term, Σext;;; [] |- v ⇝ℇ v' ∧
-  ∥ Ee.eval (strip_env Σ') (strip Σ' t') (strip Σ' v') ∥.
-Proof.
-  intros Σext wt.
-  intros HΣ' Ht' etaΣ' etat' ev.
-  pose proof (erases_erase wt); eauto.
-  rewrite HΣ' in H.
-  destruct wt as [T wt].
-  destruct wfext as [wf].
-  assert (includes_deps Σ Σ' (term_global_deps t')).
-  { rewrite <- Ht'.
-    eapply erase_global_includes.
-    intros.
-    eapply term_global_deps_spec in H; eauto.
-    eapply KernameSet.subset_spec.
-    intros x hin; auto. }
-  pose proof (erase_global_erases_deps wf wt H H0).
-  eapply (ErasureCorrectness.erases_correct Σext) in ev as [v' [ev evv]]; tea.
-  exists v'. split => //.
-  sq. apply strip_eval; tea.
-  subst Σ'; eapply erase_global_closed; tea.  
-  subst Σ'; eapply erase_global_wf_glob; tea.
-  clear HΣ'. eapply PCUICClosedTyp.subject_closed in wt.
-  eapply erases_closed in H; tea.  
-Qed.
-
-Lemma strip_fast_correct (wfl := Ee.default_wcbv_flags) (Σ : wf_env) univs wfext t v Σ' t' :
-  let Σext := make_wf_env_ext Σ univs wfext in
-  forall wt : welltyped Σext [] t,
-  erase Σext [] t wt = t' ->
-  erase_global (term_global_deps t') Σ = Σ' ->
-  isEtaExp_env Σ' ->
-  isEtaExp Σ' t' ->
-  PCUICWcbvEval.eval Σ t v ->
-  ∃ v' : term, Σext;;; [] |- v ⇝ℇ v' ∧ 
-  ∥ Ee.eval (Fast.strip_env Σ') (Fast.strip Σ' [] t') (Fast.strip Σ' [] v') ∥.
-Proof.
-  intros Σext wt ?????.
-  eapply strip_correct in X; tea.
-  destruct X as [v' [er [ev]]]. exists v'; split => //.
-  split. now rewrite -!Fast.strip_fast -Fast.strip_env_fast.
-Qed.*)
