erasure/theories/EWcbvEval.v
@@ -2,7 +2,7 @@
 From Coq Require Import Program.
 From MetaCoq.Template Require Import config utils.
 From MetaCoq.PCUIC Require PCUICWcbvEval.
-From MetaCoq.Erasure Require Import EAst EAstUtils ELiftSubst ECSubst EReflect ETyping.
+From MetaCoq.Erasure Require Import EAst EAstUtils ELiftSubst ECSubst EReflect EGlobalEnv.
 
 From Equations Require Import Equations.
 Require Import ssreflect ssrbool.
@@ -71,10 +71,11 @@ Definition cunfold_cofix (mfix : mfixpoint term) (idx : nat) :=
   end.
 
 (* Tells if the evaluation relation should include match-prop and proj-prop reduction rules. *)
-Class WcbvFlags := { with_prop_case : bool }.
+Class WcbvFlags := { with_prop_case : bool ; with_guarded_fix : bool }.
 
-Definition default_wcbv_flags := {| with_prop_case := true |}.
-Definition opt_wcbv_flags := {| with_prop_case := false |}.
+Definition default_wcbv_flags := {| with_prop_case := true ; with_guarded_fix := true |}.
+Definition opt_wcbv_flags := {| with_prop_case := false ; with_guarded_fix := true |}.
+Definition target_wcbv_flags := {| with_prop_case := false ; with_guarded_fix := false |}.
 
 Section Wcbv.
   Context {wfl : WcbvFlags}.
@@ -121,6 +122,7 @@ Section Wcbv.
 
   (** Fix unfolding, with guard *)
   | eval_fix f mfix idx argsv a av fn res :
+      forall guarded : with_guarded_fix,
       eval f (mkApps (tFix mfix idx) argsv) ->
       eval a av ->
       cunfold_fix mfix idx = Some (#|argsv|, fn) ->
@@ -129,11 +131,21 @@ Section Wcbv.
 
   (** Fix stuck, with guard *)
   | eval_fix_value f mfix idx argsv a av narg fn :
+      forall guarded : with_guarded_fix,
       eval f (mkApps (tFix mfix idx) argsv) ->
       eval a av ->
       cunfold_fix mfix idx = Some (narg, fn) ->
       (#|argsv| < narg) ->
       eval (tApp f a) (tApp (mkApps (tFix mfix idx) argsv) av)
+
+  (** Fix unfolding, without guard *)
+  | eval_fix' f mfix idx a av fn res narg :
+    forall unguarded : with_guarded_fix = false,
+    eval f (tFix mfix idx) ->
+    cunfold_fix mfix idx = Some (narg, fn) ->
+    eval a av ->
+    eval (tApp fn av) res ->
+    eval (tApp f a) res
 
   (** CoFix-case unfolding *)
   | eval_cofix_case ip mfix idx args discr narg fn brs res :
@@ -172,7 +184,7 @@ Section Wcbv.
   (** Atoms (non redex-producing heads) applied to values are values *)
   | eval_app_cong f f' a a' :
       eval f f' ->
-      ~~ (isLambda f' || isFixApp f' || isBox f') ->
+      ~~ (isLambda f' || (if with_guarded_fix then isFixApp f' else isFix f') || isBox f') ->
       eval a a' ->
       eval (tApp f a) (tApp f' a')
 
@@ -208,7 +220,7 @@ Section Wcbv.
   Inductive value : term -> Type :=
   | value_atom t : atom t -> value t
   | value_app t l : value_head t -> All value l -> value (mkApps t l)
-  | value_stuck_fix f args :
+  | value_stuck_fix f args (guarded : with_guarded_fix) :
       All value args ->
       isStuckFix f args ->
       value (mkApps f args)
@@ -217,7 +229,7 @@ Section Wcbv.
   Lemma value_values_ind : forall P : term -> Type,
       (forall t, atom t -> P t) ->
       (forall t l, value_head t -> All value l -> All P l -> P (mkApps t l)) ->
-      (forall f args,
+      (forall f args (guarded : with_guarded_fix),
           All value args ->
           All P args ->
           isStuckFix f args ->
@@ -250,7 +262,7 @@ Section Wcbv.
   Lemma value_mkApps_inv t l :
     ~~ isApp t ->
     value (mkApps t l) ->
-    ((l = []) × atom t) + (value_head t × All value l) + (isStuckFix t l × All value l).
+    ((l = []) × atom t) + (value_head t × All value l) + (with_guarded_fix × isStuckFix t l × All value l).
   Proof.
     intros H H'. generalize_eqs H'. revert t H. induction H' using value_values_ind.
     intros.
@@ -287,12 +299,12 @@ Section Wcbv.
       apply value_mkApps_inv in IHeval1; [|easy].
       destruct IHeval1 as [[(-> & _)|]|(stuck & vals)].
       + cbn in *.
-        apply (value_stuck_fix _ [av]); [easy|].
+        apply (value_stuck_fix _ [av]); [eauto|easy|].
         cbn.
         destruct (cunfold_fix mfix idx) as [(? & ?)|]; [|easy].
         noconf e. destruct narg; auto. lia.
       + easy.
-      + eapply value_stuck_fix; [now apply All_app_inv|].
+      + eapply value_stuck_fix;  [easy | now apply All_app_inv|].
         unfold isStuckFix in *.
         destruct (cunfold_fix mfix idx) as [(? & ?)|]; [|easy].
         noconf e. rewrite app_length; simpl.
@@ -303,15 +315,17 @@ Section Wcbv.
       destruct IHeval1; intuition subst.
       * rewrite -> a1 in *.
         simpl in *.
-        apply (value_app f0 [a']). destruct f0; simpl in * |- *; try congruence.
-        constructor; auto. constructor. constructor; auto.
+        apply (value_app f0 [a']). destruct with_guarded_fix;
+        destruct f0; simpl in * |- *; try congruence;
+           constructor; auto. constructor; eauto. 
       * rewrite -[tApp _ _](mkApps_app _ (firstn n l) [a']).
         constructor 2; auto. eapply All_app_inv; auto.
       * rewrite -[tApp _ _](mkApps_app _ (firstn n l) [a']).
         erewrite isFixApp_mkApps in i => //.
         destruct f0; simpl in *; try congruence.
         rewrite /isFixApp in i. simpl in i.
-        rewrite orb_true_r orb_true_l in i. easy.
+        rewrite a0 in i.
+        rewrite orb_true_r orb_true_l in i. easy.         
   Qed.
 
   Lemma closed_fix_substl_subst_eq {mfix idx d} : 
@@ -403,6 +417,29 @@ Section Wcbv.
       * easy.
   Qed.
 
+  
+  Lemma eval_mkApps_tFix_inv mfix idx args v :
+   with_guarded_fix ->
+    eval (mkApps (tFix mfix idx) args) v ->
+    (exists args', v = mkApps (tFix mfix idx) args' /\ #|args| = #|args'|) \/
+    (exists n b, cunfold_fix mfix idx = Some (n, b) /\ n < #|args|).
+  Proof.
+    revert v.
+    induction args using List.rev_ind; intros wg v ev.
+    + left. exists [].
+      now depelim ev.
+    + rewrite mkApps_app in ev.
+      cbn in *.
+      depelim ev.
+      all: try (eapply IHargs in ev1 as [(? & ? & Heq) | (? & ? & ? & ?)]; eauto; rewrite ?Heq; try solve_discr;
+        len; rewrite ?Heq; rewrite Nat.add_comm; eauto 7).
+      * invs H. eauto 9.
+      * invs H. left. exists (x0 ++ [av]). rewrite mkApps_app. cbn. split. eauto. len. 
+      * subst. rewrite isFixApp_mkApps in i => //. rewrite v in i. cbn in i.
+        destruct isLambda; cbn in i; easy.
+      * invs i.
+  Qed.
+
   Derive NoConfusionHom for EAst.global_decl.
 
   Lemma Forall_Forall2_refl :
@@ -413,18 +450,21 @@ Section Wcbv.
   Qed.
 
   Lemma value_head_spec_impl t :
-    implb (value_head t) (~~ (isLambda t || isFixApp t || isBox t)).
+    implb (value_head t) (~~ (isLambda t || (if with_guarded_fix then isFixApp t else isFix t) || isBox t)).
   Proof.
-    destruct t; simpl; intuition auto; eapply implybT.
+    destruct with_guarded_fix;
+    destruct t; simpl; intuition auto; eapply implyb.
   Qed.
 
   Derive Signature for Forall.
 
   Lemma eval_stuck_fix args argsv mfix idx :
+    with_guarded_fix ->
     All2 eval args argsv ->
     isStuckFix (tFix mfix idx) argsv ->
     eval (mkApps (tFix mfix idx) args) (mkApps (tFix mfix idx) argsv).
   Proof.
+    intros guarded.
     revert argsv.
     induction args as [|a args IH] using MCList.rev_ind;
     intros argsv all stuck.
@@ -438,7 +478,8 @@ Section Wcbv.
       cbn in *.
       destruct (cunfold_fix mfix idx) as [(? & ?)|] eqn:cuf; [|easy].
       eapply eval_fix_value.
-      + apply IH; [easy|].
+      + easy.
+      + eapply IH; [easy|].
         destruct (cunfold_fix mfix idx) as [(? & ?)|]; [|easy].
         rewrite app_length /= in stuck.
         eapply Nat.leb_le in stuck. eapply Nat.leb_le. lia.
@@ -497,11 +538,11 @@ Section Wcbv.
         eapply value_head_nApp in H.
         rewrite isFixApp_mkApps => //.
         rewrite mkApps_app; simpl.
-        rewrite orb_false_r.
+        destruct with_guarded_fix => //.
         destruct t => //.
     - destruct f; try discriminate.
       apply All_All2_refl in X0.
-      now apply eval_stuck_fix.
+      eapply eval_stuck_fix; eauto.
   Qed.
 
   Set Equations With UIP.
@@ -523,7 +564,10 @@ Section Wcbv.
     intros ev.
     revert v'.
     depind ev; intros v' ev'.
-    - depelim ev'; go.
+    - depelim ev'; try go.
+      specialize (IHev1 _ ev'1). noconf IHev1.
+      specialize (IHev2 _ ev'2). noconf IHev2. cbn in i. 
+      exfalso. destruct (@with_guarded_fix wfl); easy.
     - depelim ev'; go.
     - depelim ev'; go.
     - depelim ev'; try go.
@@ -554,7 +598,8 @@ Section Wcbv.
         specialize (IHev2 _ ev'2); noconf IHev2.
         assert (fn0 = fn) as -> by congruence.
         assert (e0 = e) as -> by now apply uip.
-        now specialize (IHev3 _ ev'3); noconf IHev3.
+        rewrite (uip guarded guarded0).
+        now specialize (IHev3 _ ev'3); noconf IHev3.        
       + specialize (IHev1 _ ev'1).
         pose proof (mkApps_eq_inj (f_equal pr1 IHev1) eq_refl eq_refl) as (? & <-).
         noconf H.
@@ -564,8 +609,8 @@ Section Wcbv.
       + specialize (IHev1 _ ev'1).
         noconf IHev1.
         exfalso.
-        rewrite isFixApp_mkApps in i by easy.
-        cbn in *.
+        rewrite guarded in i.
+        rewrite isFixApp_mkApps in i; try easy.
         now rewrite Bool.orb_true_r in i.
     - depelim ev'; try go.
       + specialize (IHev1 _ ev'1).
@@ -582,24 +627,27 @@ Section Wcbv.
         assert (narg0 = narg) as -> by congruence.
         assert (fn0 = fn) as -> by congruence.
         assert (e0 = e) as -> by now apply uip.
+        rewrite (uip guarded guarded0).
         now assert (l0 = l) as -> by now apply PCUICWcbvEval.le_irrel.
       + specialize (IHev1 _ ev'1).
         noconf IHev1.
-        exfalso.
-        rewrite isFixApp_mkApps in i by easy.
+        exfalso.  rewrite guarded in i.
+        rewrite isFixApp_mkApps in i; try easy.
         cbn in *.
         now rewrite Bool.orb_true_r in i.
     - depelim ev'; try go.
-      move: (IHev1 _ ev'1).
-      eapply DepElim.simplification_sigma1 => heq IHev1'.
-      apply mkApps_eq_inj in heq as H'; auto.
-      destruct H' as (H' & <-). noconf H'.
-      assert (narg0 = narg) as -> by congruence.
-      assert (fn0 = fn) as -> by congruence.
-      noconf IHev1'.
-      assert (e0 = e) as -> by now apply uip.
-      cbn in *; subst.
-      now specialize (IHev2 _ ev'2); noconf IHev2.
+      + move: (IHev1 _ ev'1).
+        eapply DepElim.simplification_sigma1 => heq IHev1'.
+        assert (narg0 = narg) as -> by congruence.
+        assert (fn0 = fn) as -> by congruence.
+        noconf IHev1'.
+        assert (e0 = e) as -> by now apply uip.
+        rewrite (uip unguarded unguarded0).
+        cbn in *; subst.
+        specialize (IHev2 _ ev'2). noconf IHev2.
+        now specialize (IHev3 _ ev'3); noconf IHev3.
+      + exfalso. rewrite unguarded in i.
+        specialize (IHev1 _ ev'1). depelim IHev1. easy.
     - depelim ev'; try go.
       move: (IHev1 _ ev'1).
       eapply DepElim.simplification_sigma1 => heq IHev1'.
@@ -612,7 +660,18 @@ Section Wcbv.
       cbn in *; subst.
       now specialize (IHev2 _ ev'2); noconf IHev2.
     - depelim ev'; try go.
-      unfold ETyping.declared_constant in *.
+      move: (IHev1 _ ev'1).
+      eapply DepElim.simplification_sigma1 => heq IHev1'.
+      apply mkApps_eq_inj in heq as H'; auto.
+      destruct H' as (H' & <-). noconf H'.
+      assert (narg0 = narg) as -> by congruence.
+      assert (fn0 = fn) as -> by congruence.
+      noconf IHev1'.
+      assert (e0 = e) as -> by now apply uip.
+      cbn in *; subst.
+      now specialize (IHev2 _ ev'2); noconf IHev2.
+    - depelim ev'; try go.
+      unfold EGlobalEnv.declared_constant in *.
       assert (decl0 = decl) as -> by congruence.
       assert (body0 = body) as -> by congruence.
       assert (e0 = e) as -> by now apply uip.
@@ -631,15 +690,21 @@ Section Wcbv.
       now rewrite (uip i0 i2).
     - depelim ev'; try go.
       + specialize (IHev1 _ ev'1); noconf IHev1.
+        exfalso; destruct with_guarded_fix; cbn in *; easy.
+      + specialize (IHev1 _ ev'1); noconf IHev1.
         exfalso.
-        rewrite isFixApp_mkApps in i by easy.
+        rewrite isFixApp_mkApps in i; try easy.
         cbn in *.
+        destruct with_guarded_fix; try easy.
         now rewrite Bool.orb_true_r in i.
       + specialize (IHev1 _ ev'1); noconf IHev1.
         exfalso.
-        rewrite isFixApp_mkApps in i by easy.
+        rewrite isFixApp_mkApps in i; try easy.
         cbn in *.
+        destruct with_guarded_fix; try easy.
         now rewrite Bool.orb_true_r in i.
+      + specialize (IHev1 _ ev'1); noconf IHev1.
+        exfalso. rewrite unguarded in i. easy.
       + specialize (IHev1 _ ev'1); noconf IHev1.
         specialize (IHev2 _ ev'2); noconf IHev2.
         now assert (i0 = i) as -> by now apply uip.
@@ -656,7 +721,16 @@ Section Wcbv.
     pose proof (eval_unique_sig ev ev').
     now noconf H.
   Qed.
-
+  
+  Lemma eval_trans {e e' e''} :
+    eval e e' -> eval e' e'' -> e' = e''.
+  Proof.
+    intros ev ev'.
+    eapply eval_to_value in ev.
+    eapply value_final in ev.
+    eapply (eval_deterministic ev ev').
+  Qed.
+  
   Lemma eval_unique {t v} :
     forall (ev1 : eval t v) (ev2 : eval t v),
       ev1 = ev2.
@@ -693,6 +767,10 @@ Section Wcbv.
         exists f'; split => //.
         rewrite mkApps_app.
         eapply eval_fix_value; tea.
+      + specialize (IHargs _ _ ev1) as [f' [evf' ev]].
+        exists f'; split => //.
+        rewrite mkApps_app.
+        eapply eval_fix'; eauto.
       + specialize (IHargs _ _ ev1) as [f'' [evf' ev]].
         exists f''; split => //.
         rewrite mkApps_app.
@@ -701,6 +779,53 @@ Section Wcbv.
   Qed.
 
 End Wcbv.
+
+(*
+Lemma eval_mkApps_inv' Σ f args v :
+  @eval target_wcbv_flags Σ (mkApps f args) v ->
+  ∑ f', @eval target_wcbv_flags Σ f f' × ∑ args', All2 (@eval target_wcbv_flags  Σ) args args' × @eval target_wcbv_flags Σ (mkApps f' args') v.
+Proof.
+  revert f v; induction args using rev_ind; cbn; intros f v.
+  - intros ev. exists v. split => //. eapply eval_to_value in ev.
+    exists []. split. econstructor. cbn.
+    now eapply value_final.
+  - rewrite mkApps_app. intros ev.
+    depelim ev.
+    + specialize (IHargs _ _ ev1) as [f' [evf' [args' [Hargs' evars]]]].
+      exists f'. split => //.
+      eexists. split. eapply All2_app; eauto.
+      rewrite mkApps_app.
+      econstructor; tea.
+      eapply value_final; eapply eval_to_value; eauto.
+    + specialize (IHargs _ _ ev1) as [f' [evf' [args' [Hargs' evars]]]].
+      exists f'. split => //.
+      eexists. split. eapply All2_app; eauto.
+      rewrite mkApps_app. 
+      eapply eval_beta; tea.
+      eapply value_final; eapply eval_to_value; eauto.
+    + specialize (IHargs _ _ ev1) as [f' [evf' ev]].
+      exists f'; split => //. (* 
+      rewrite mkApps_app.
+      eapply eval_fix; tea. *)
+    + specialize (IHargs _ _ ev1) as [f' [evf' ev]].
+      exists f'; split => //.
+      (* rewrite mkApps_app.
+      eapply eval_fix_value; tea. *)
+    + specialize (IHargs _ _ ev1) as [f' [evf' [args' [Hargs' evars]]]].
+      exists f'. split => //.
+      eexists. split. eapply All2_app; eauto.>
+      rewrite mkApps_app. 
+    
+    specialize (IHargs _ _ ev1) as [f' [evf' ev]].
+      exists f'; split => //.
+      rewrite mkApps_app.
+      eapply eval_fix'; eauto.
+    + specialize (IHargs _ _ ev1) as [f'' [evf' ev]].
+      exists f''; split => //.
+      rewrite mkApps_app.
+      eapply eval_app_cong; tea.
+    + cbn in i. discriminate.
+Qed.*)
 
 Arguments eval_unique_sig {_ _ _ _ _}.
 Arguments eval_deterministic {_ _ _ _ _}.
@@ -721,3 +846,337 @@ Section WcbvEnv.
 
 End WcbvEnv.
 
+Scheme eval_nondep := Minimality for eval Sort Prop.
+
+Fixpoint eval_depth {wfl : WcbvFlags} {Σ : EAst.global_declarations} {t1 t2 : EAst.term} (ev : eval Σ t1 t2) { struct ev } : nat.
+Proof.
+  rename eval_depth into aux.
+  destruct ev.
+  all:try match goal with
+  | [ H : eval _ _ _, H' : eval _ _ _, H'' : eval _ _ _ |- _ ] => 
+    apply aux in H; apply aux in H'; apply aux in H''; exact (S (Nat.max H (Nat.max H' H'')))
+  | [ H : eval _ _ _, H' : eval _ _ _ |- _ ] => 
+    apply aux in H; apply aux in H'; exact (S (Nat.max H H'))
+  | [ H : eval _ _ _ |- _ ] => apply aux in H; exact (S H)
+  end.
+  exact 1.
+Defined.
+
+Lemma eval_construct_size  {fl : WcbvFlags} [Σ kn c args e] : 
+  forall (ev : eval Σ (mkApps (tConstruct kn c) args) e),
+  ∑ args', (e = mkApps (tConstruct kn c) args') ×
+  All2 (fun x y => ∑ ev' : eval Σ x y, eval_depth ev' < eval_depth ev) args args'.
+Proof.
+  revert e; induction args using rev_ind; intros e.
+  - intros ev. depelim ev. exists []=> //.
+  - intros ev. revert ev.
+    rewrite mkApps_app /=.
+    intros ev.
+    depelim ev; try solve_discr.
+    destruct (IHargs _ ev1) as [? []]. solve_discr.
+    all:try specialize (IHargs _ ev1) as [? []]; try solve_discr.
+    * subst f'. 
+      exists (x0 ++ [a'])%list.
+      rewrite mkApps_app /= //.
+      cbn in i. split => //. eapply All2_app; eauto.
+      eapply All2_impl; tea. cbn. intros ? ? [ev' ?]. exists ev'. lia.
+      constructor. exists ev2. lia. constructor.
+    * now cbn in i.
+Qed.
+
+Lemma eval_mkApps_Construct {fl : WcbvFlags} Σ kn c args args' : 
+  All2 (eval Σ) args args' ->
+  eval Σ (mkApps (tConstruct kn c) args) (mkApps (tConstruct kn c) args').
+Proof.
+  revert args'. induction args using rev_ind; intros args'; destruct args' using rev_case; intros a.
+  - depelim a. constructor => //.
+  - depelim a. cbn. now apply app_tip_nil in H.
+  - depelim a. now apply app_tip_nil in H.
+  - eapply All2_app_inv in a as []. 2:{ eapply All2_length in a. len in a. cbn in a. lia. } 
+    depelim a0. clear a0. rewrite !mkApps_app /=.
+    constructor; auto.
+    destruct args' using rev_ind; try now rewrite ?mkApps_app; cbn; destruct with_guarded_fix; eauto.
+    cbn. rewrite isFixApp_mkApps; eauto.
+    cbn. try now rewrite ?mkApps_app; cbn; destruct with_guarded_fix; eauto.
+Qed.
+
+Require Import Utf8.
+From MetaCoq.Template Require Import BasicAst.
+
+
+Lemma isLambda_mkApps f l : ~~ isLambda f -> ~~ EAst.isLambda (mkApps f l).
+Proof.
+  induction l using rev_ind; simpl; auto => //.
+  intros isf; specialize (IHl isf).
+  now rewrite mkApps_app.
+Qed.
+
+Lemma isBox_mkApps f l : ~~ isBox f -> ~~ isBox (mkApps f l).
+Proof.
+  induction l using rev_ind; simpl; auto => //.
+  intros isf; specialize (IHl isf).
+  now rewrite mkApps_app.
+Qed.
+
+
+Lemma closedn_mkApps k f args : closedn k (mkApps f args) = closedn k f && forallb (closedn k) args.
+Proof.
+  induction args in f |- *; simpl; auto.
+  ring. rewrite IHargs /=. ring. 
+Qed.
+
+Lemma closed_fix_subst mfix : 
+  forallb (EAst.test_def (closedn (#|mfix| + 0))) mfix ->
+  forallb (closedn 0) (fix_subst mfix).
+Proof.
+  solve_all.
+  unfold fix_subst.
+  move: #|mfix| => n.
+  induction n. constructor.
+  cbn. rewrite H IHn //.
+Qed.
+
+Lemma closed_cofix_subst mfix : 
+  forallb (EAst.test_def (closedn (#|mfix| + 0))) mfix ->
+  forallb (closedn 0) (cofix_subst mfix).
+Proof.
+  solve_all.
+  unfold cofix_subst.
+  move: #|mfix| => n.
+  induction n. constructor.
+  cbn. rewrite H IHn //.
+Qed.
+
+Lemma closed_cunfold_fix mfix idx n f : 
+  closed (EAst.tFix mfix idx) ->
+  cunfold_fix mfix idx = Some (n, f) ->
+  closed f.
+Proof.
+  move=> cl.
+  rewrite /cunfold_fix.
+  destruct nth_error eqn:heq => //.
+  cbn in cl.
+  have := (nth_error_forallb heq cl) => cld. 
+  move=> [=] _ <-.
+  eapply closed_substl. now eapply closed_fix_subst.
+  rewrite fix_subst_length.
+  apply cld.
+Qed.
+
+Lemma closed_cunfold_cofix mfix idx n f : 
+  closed (EAst.tCoFix mfix idx) ->
+  cunfold_cofix mfix idx = Some (n, f) ->
+  closed f.
+Proof.
+  move=> cl.
+  rewrite /cunfold_cofix.
+  destruct nth_error eqn:heq => //.
+  cbn in cl.
+  have := (nth_error_forallb heq cl) => cld. 
+  move=> [=] _ <-.
+  eapply closed_substl. now eapply closed_cofix_subst.
+  rewrite cofix_subst_length.
+  apply cld.
+Qed.
+
+Lemma lookup_env_closed {Σ kn decl} : EGlobalEnv.closed_env Σ -> EGlobalEnv.lookup_env Σ kn = Some decl -> EGlobalEnv.closed_decl decl.
+Proof.
+  induction Σ; cbn => //.
+  move/andP => [] cla cle.
+  destruct (eqb_spec kn a.1).
+  move=> [= <-]. apply cla.
+  now eapply IHΣ.
+Qed.
+
+(** Evaluation preserves closedness: *)
+Lemma eval_closed {wfl : WcbvFlags} Σ : 
+  closed_env Σ ->
+  forall t u, closed t -> eval Σ t u -> closed u.
+Proof.
+  move=> clΣ t u Hc ev. move: Hc.
+  induction ev; simpl in *; auto;
+    (move/andP=> [/andP[Hc Hc'] Hc''] || move/andP=> [Hc Hc'] || move=>Hc); auto.
+  - eapply IHev3. rewrite ECSubst.closed_subst //. auto.
+    eapply closedn_subst; tea. cbn. rewrite andb_true_r. auto. cbn. auto.
+  - eapply IHev2.
+    rewrite ECSubst.closed_subst; auto.
+    eapply closedn_subst; tea. cbn. rewrite andb_true_r. auto.
+  - specialize (IHev1 Hc).
+    move: IHev1; rewrite closedn_mkApps => /andP[] _ clargs.
+    apply IHev2. rewrite /iota_red.
+    eapply closed_substl. now rewrite forallb_rev forallb_skipn.
+    len.
+    rewrite e1. eapply nth_error_forallb in Hc'; tea.
+    now rewrite Nat.add_0_r in Hc'.
+  - subst brs. cbn in Hc'. rewrite andb_true_r in Hc'.
+    eapply IHev2. eapply closed_substl.
+    eapply All_forallb, All_repeat => //.
+    now rewrite repeat_length.
+  - eapply IHev3.
+    apply/andP.
+    split; [|easy].
+    specialize (IHev1 Hc).
+    rewrite closedn_mkApps in IHev1.
+    move/andP: IHev1 => [clfix clargs].
+    rewrite closedn_mkApps clargs andb_true_r.
+    eapply closed_cunfold_fix; tea.
+  - apply andb_true_iff.
+    split; [|easy].
+    solve_all.
+  - eapply IHev3. rtoProp. split; eauto.
+    eapply closed_cunfold_fix; tea. eauto.
+  - eapply IHev2. rewrite closedn_mkApps.
+    rewrite closedn_mkApps in IHev1. 
+    specialize (IHev1 Hc). move/andP: IHev1 => [Hfix Hargs].
+    repeat (apply/andP; split; auto).
+    eapply closed_cunfold_cofix; tea. 
+  - specialize (IHev1 Hc). eapply IHev2. rewrite closedn_mkApps in IHev1 *.
+     move/andP: IHev1 => [Hfix Hargs].
+    rewrite closedn_mkApps Hargs.
+    rewrite andb_true_r.
+    eapply closed_cunfold_cofix; tea.
+  - apply IHev.
+    move/(lookup_env_closed clΣ): isdecl.
+    now rewrite /closed_decl e /=.
+  - have := (IHev1 Hc).
+    rewrite closedn_mkApps /= => clargs.
+    eapply IHev2; eauto.
+    rewrite nth_nth_error.
+    destruct nth_error eqn:hnth => //.
+    eapply nth_error_forallb in clargs; tea.
+  - rtoProp; intuition auto.
+Qed.
+
+
+Lemma remove_last_length {X} {l : list X} : 
+  #|remove_last l| = match l with nil => 0 | _ => #|l| - 1 end.
+Proof.
+  unfold remove_last. rewrite firstn_length.
+  destruct l; cbn; lia.
+Qed.
+
+Lemma remove_last_length' {X} {l : list X} : 
+  l <> nil -> 
+  #|remove_last l| = #|l| - 1.
+Proof.
+  intros. rewrite remove_last_length. destruct l; try congruence; lia.
+Qed.
+ 
+Local Hint Rewrite @remove_last_length : len.
+
+Lemma eval_mkApps_tFix_inv_size {wfl : WcbvFlags} Σ mfix idx args v :
+  with_guarded_fix ->
+  forall Heval : eval Σ (mkApps (tFix mfix idx) args) v,
+  (∑ args', All2 (fun a a' => ∑ H : eval Σ a a', eval_depth H < eval_depth Heval) args args' × v = mkApps (tFix mfix idx) (args')) +
+  (∑ n b, args <> nil /\ cunfold_fix mfix idx = Some (n, b) /\ n < #|args|).
+Proof.
+ revert v.
+ induction args using rev_ind; intros v wg ev.
+ + left. exists []. split. repeat econstructor. now depelim ev.
+ + rewrite mkApps_app in ev |- *.
+   cbn in *.
+   depelim ev.
+  
+   all: try(specialize (IHargs) with (Heval := ev1); destruct IHargs as [(args' & ? & Heq) | (? & ? & ? & ? & ?)];eauto; rewrite ?Heq; try solve_discr; try congruence;
+     len; rewrite ?Heq; rewrite Nat.add_comm; eauto 9).
+   * right. repeat eexists. destruct args; cbn; congruence. eauto. lia.
+   * right. repeat eexists. destruct args; cbn; congruence. eauto. lia.
+   * invs H. eapply All2_length in a. right. repeat eexists. destruct args; cbn; congruence. eauto. lia.
+   * right. repeat eexists. destruct args; cbn; congruence. eauto. lia.
+   * invs H. left. eexists. split. sq. eapply All2_app. solve_all. destruct H. unshelve eexists. eauto. cbn. lia.
+     econstructor. 2: econstructor.
+     unshelve eexists. eauto. lia.
+     now rewrite !mkApps_app.
+   * right. repeat eexists. destruct args; cbn; congruence. eauto. lia.
+   * subst. sq.  rewrite wg in i. rewrite isFixApp_mkApps in i => //. cbn in i. destruct EAst.isLambda; easy.
+   * right. repeat eexists. destruct args; cbn; congruence. eauto. lia.
+   * inv i.
+Qed.
+
+Lemma size_final {wfl : WcbvFlags} Σ t v :
+  forall He : eval Σ t v, ∑ He' : eval Σ v v, eval_depth He' <= eval_depth He.
+Proof.
+  intros He. induction He.
+  all: try now unshelve eexists; eauto; [ eapply IHHe | cbn; destruct IHHe; lia ].
+  all: try now unshelve eexists; eauto; [ eapply IHHe2 | cbn; destruct IHHe2; lia ].
+  all: try now unshelve eexists; eauto; [ eapply IHHe3 | cbn; destruct IHHe3; lia ].
+  all: try now unshelve eexists; eauto; cbn; lia.
+  - unshelve eexists. repeat econstructor. cbn; lia.
+  - unshelve eexists; eauto. eapply eval_fix_value; eauto. eapply IHHe1. eapply IHHe2. cbn. destruct IHHe1, IHHe2. lia.
+  - unshelve eexists. eapply eval_app_cong; eauto. eapply IHHe1. eapply IHHe2. cbn. destruct IHHe1, IHHe2. lia.
+Qed.
+
+Lemma eval_mkApps_tFix_inv_size_unguarded {wfl : WcbvFlags} Σ mfix idx args v :
+  with_guarded_fix = false ->
+  forall Heval : eval Σ (mkApps (tFix mfix idx) args) v,
+  (args = [] /\ v = tFix mfix idx)
+  + ∑ a av args' argsv, 
+    (args = a :: args')%list ×
+    All2 (fun a a' => (a = a') + (∑ H : eval Σ a a', eval_depth H < eval_depth Heval)) args' argsv ×
+    ∑ n fn, cunfold_fix mfix idx = Some (n, fn) ×
+    ∑ H : eval Σ a av, eval_depth H <= eval_depth Heval ×
+    ∑ H : eval Σ (mkApps (tApp fn av) argsv) v, eval_depth H <= eval_depth Heval.
+Proof.
+ revert v.
+ induction args using rev_ind; intros v wg ev.
+ + left. now depelim ev.
+ + rewrite mkApps_app in ev |- *.
+   cbn in *.
+   depelim ev; right.
+  
+   all: try(specialize (IHargs) with (Heval := ev1); destruct IHargs as [[-> Heq] | (a & aval & args' & argsv_ & Heqargs & Hall & n & fn_ & Hunf & Heva & Hevasz & Hev' & Hevsz')];eauto; try rewrite ?Heq; try solve_discr; try congruence;
+     len; try rewrite ?Heq; rewrite ?Nat.add_comm; eauto 9).
+   * subst. cbn. exists a, aval, (args' ++ [x])%list,(argsv_ ++ [t'])%list. split. reflexivity.
+      repeat unshelve eexists; eauto. 3:{ rewrite mkApps_app. econstructor. eauto. eapply size_final. eauto. }
+      eapply All2_app.
+      solve_all. right. destruct b. unshelve eexists; eauto. lia.
+      unshelve econstructor. right. unshelve eexists. eauto. lia. repeat econstructor.
+      cbn in *; lia.
+      cbn. generalize (mkApps_app (tApp fn_ aval) argsv_ [t']). generalize (EAst.mkApps (tApp fn_ aval) (argsv_ ++ [t'])).
+      cbn. intros. subst. cbn. destruct size_final. cbn in *. lia.
+   * subst. cbn. exists a, aval, (args' ++ [x])%list,(argsv_ ++ [a'])%list. split. reflexivity.
+     repeat unshelve eexists; eauto.
+     eapply All2_app.
+     solve_all. right. destruct b0. unshelve eexists; eauto. lia.
+   unshelve econstructor. right. unshelve eexists. eauto. lia. repeat econstructor.
+   cbn in *; lia.
+   rewrite mkApps_app. cbn. econstructor; eauto. eapply size_final; eauto.
+   cbn. generalize (mkApps_app (tApp fn_ aval) argsv_ [a']). generalize (EAst.mkApps (tApp fn_ aval) (argsv_ ++ [a'])).
+   intros. subst. cbn.
+   destruct size_final. cbn in *. lia.
+  
+   * invs Heq. exists x, av, [], []. repeat split. econstructor. repeat unshelve eexists; eauto.
+     all:cbn; lia.
+   * subst. cbn. eexists _, _, _, (argsv_ ++ [_])%list. repeat eexists. 2: eauto.
+    eapply All2_app.
+     solve_all. right. destruct b. exists x1. cbn. lia. econstructor. now left. econstructor.
+     Unshelve. 5:{ rewrite mkApps_app. eapply eval_fix'; eauto. }
+     3:tea. cbn in *; lia.
+     cbn. generalize (mkApps_app (tApp fn_ aval) argsv_ [x]). generalize (EAst.mkApps (tApp fn_ aval) (argsv_ ++ [x])). intros. subst. cbn.
+     cbn in *. lia.
+   * subst. cbn in i. exfalso. destruct with_guarded_fix; easy.
+   * subst.  cbn. eexists _, _, _, (argsv_ ++ [_])%list. repeat eexists. 2: eauto.
+     eapply All2_app.
+     solve_all. right. destruct b. exists x1. cbn. lia. econstructor. now left. econstructor.
+     Unshelve. 4:tea. 3:{ rewrite mkApps_app. eapply eval_app_cong; eauto. }
+     cbn in *; lia.
+     cbn. generalize (mkApps_app (tApp fn_ aval) argsv_ [x]). generalize (EAst.mkApps (tApp fn_ aval) (argsv_ ++ [x])). intros. subst. cbn.
+     cbn in *. lia.
+   * subst. cbn. invs i.
+Qed.
+
+Lemma eval_construct  {fl : WcbvFlags} Σ kn c args e : 
+  eval Σ (mkApps (tConstruct kn c) args) e -> ∑ args', (e = mkApps (tConstruct kn c) args') × All2 (eval Σ) args args'.
+Proof.
+  revert e; induction args using rev_ind; intros e.
+  - intros ev. depelim ev. exists []=> //.
+  - intros ev. rewrite mkApps_app /= in ev.
+    depelim ev; try solve_discr.
+    destruct (IHargs _ ev1) as [? []]. solve_discr.
+    all:try specialize (IHargs _ ev1) as [? []]; try solve_discr.
+    * subst f'. 
+      exists (x0 ++ [a'])%list.
+      rewrite mkApps_app /= //.
+      cbn in i. split => //. eapply All2_app; eauto.
+    * now cbn in i.
+Qed.
