pcuic/theories/PCUICEtaExpand.v
@@ -3,92 +3,125 @@ From MetaCoq.PCUIC Require Import PCUICAst PCUICAstUtils PCUICTyping.
 Definition isConstruct t :=
    match t with tConstruct _ _ _ => true | _ => false end.
 
+ Definition isFix t :=
+  match t with tFix _ _ => true | _ => false end.
+
+Definition isRel t :=
+    match t with tRel _ => true | _ => false end.
+
 Section expanded.
 
 Variable Σ : global_env.
 
 Local Unset Elimination Schemes.
 
-Inductive expanded : term -> Prop :=
-| expanded_tRel (n : nat) : expanded (tRel n)
-| expanded_tVar (id : ident) : expanded (tVar id)
-| expanded_tEvar (ev : nat) (args : list term) : Forall expanded args -> expanded (tEvar ev args)
-| expanded_tSort (s : Universe.t) : expanded (tSort s)
-| expanded_tProd (na : aname) (ty : term) (body : term) : (* expanded ty -> expanded body -> *) expanded (tProd na ty body)
-| expanded_tLambda (na : aname) (ty : term) (body : term) : (* expanded ty ->  *)expanded body -> expanded (tLambda na ty body)
-| expanded_tLetIn (na : aname) (def : term) (def_ty : term) (body : term) : expanded def -> (* expanded def_ty ->  *)expanded body -> expanded (tLetIn na def def_ty body)
-| expanded_mkApps (f : term) (args : list term) : ~ isConstruct f -> expanded f -> Forall expanded args -> expanded (mkApps f args)
-| expanded_tConst (c : kername) (u : Instance.t) : expanded (tConst c u)
-| expanded_tInd (ind : inductive) (u : Instance.t) : expanded (tInd ind u)
+Inductive expanded (Γ : list nat) : term -> Prop :=
+| expanded_tRel (n : nat) m args : nth_error Γ n = Some m -> forall Hle : m <= #|args|, Forall (expanded Γ) args -> expanded Γ (mkApps (tRel n) args)
+| expanded_tVar (id : ident) : expanded Γ (tVar id)
+| expanded_tEvar (ev : nat) (args : list term) : Forall (expanded Γ) args -> expanded Γ (tEvar ev args)
+| expanded_tSort (s : Universe.t) : expanded Γ (tSort s)
+| expanded_tProd (na : aname) (ty : term) (body : term) : expanded Γ (tProd na ty body)
+| expanded_tLambda (na : aname) (ty : term) (body : term) : expanded (0 :: Γ) body -> expanded Γ (tLambda na ty body)
+| expanded_tLetIn (na : aname) (def : term) (def_ty : term) (body : term) : expanded Γ def -> expanded (0 :: Γ) body -> expanded Γ (tLetIn na def def_ty body)
+| expanded_mkApps (f : term) (args : list term) : ~ (isConstruct f || isFix f || isRel f) -> expanded Γ f -> Forall (expanded Γ) args -> expanded Γ (mkApps f args)
+| expanded_tConst (c : kername) (u : Instance.t) : expanded Γ (tConst c u)
+| expanded_tInd (ind : inductive) (u : Instance.t) : expanded Γ (tInd ind u)
 | expanded_tCase (ci : case_info) (type_info:predicate term)
-        (discr:term) (branches : list (branch term)) : expanded discr -> Forall (fun br => expanded br.(bbody)) branches -> expanded (tCase ci type_info discr branches)
-| expanded_tProj (proj : projection) (t : term) : expanded t -> expanded (tProj proj t)
-| expanded_tFix (mfix : mfixpoint term) (idx : nat) :   Forall (fun d => expanded d.(dtype) /\ expanded d.(dbody)) mfix -> expanded (tFix mfix idx)
-| expanded_tCoFix (mfix : mfixpoint term) (idx : nat) :   Forall (fun d => expanded d.(dtype) /\ expanded d.(dbody)) mfix -> expanded (tCoFix mfix idx)
+        (discr:term) (branches : list (branch term)) : expanded Γ discr -> Forall (fun br => expanded (repeat 0 #|br.(bcontext)| ++ Γ) br.(bbody)) branches -> expanded Γ (tCase ci type_info discr branches)
+| expanded_tProj (proj : projection) (t : term) : expanded Γ t -> expanded Γ (tProj proj t)
+| expanded_tFix (mfix : mfixpoint term) (idx : nat) args d : 
+  Forall (fun d => let ctx := rev_map (fun  d => 1 + d.(rarg)) mfix in expanded (ctx ++ Γ) d.(dbody)) mfix ->
+  Forall (expanded Γ) args ->
+  args <> [] ->
+  nth_error mfix idx = Some d ->
+  #|args| > d.(rarg) ->
+  expanded Γ (mkApps (tFix mfix idx) args)
+| expanded_tCoFix (mfix : mfixpoint term) (idx : nat) :   Forall (fun d => expanded (repeat 0 #|mfix| ++ Γ) d.(dbody)) mfix -> expanded Γ (tCoFix mfix idx)
 | expanded_tConstruct_app ind c u mind idecl cdecl args :
     declared_constructor Σ (ind, c) mind idecl cdecl ->
     #|args| >= (ind_npars mind + context_assumptions (cstr_args cdecl)) ->
-    Forall expanded args ->
-    expanded (mkApps (tConstruct ind c u) args).
+    Forall (expanded Γ) args ->
+    expanded Γ (mkApps (tConstruct ind c u) args).
 
 End expanded.
 
 Lemma expanded_ind :
-forall (Σ : global_env) (P : term -> Prop),
-(forall n : nat, P (tRel n)) ->
-(forall id : ident, P (tVar id)) ->
-(forall (ev : nat) (args : list term), Forall (expanded Σ) args -> Forall P args -> P (tEvar ev args)) ->
-(forall s : Universe.t, P (tSort s)) ->
-(forall (na : aname) (ty body : term),
-(*  expanded Σ ty -> P ty -> expanded Σ body -> P body -> *) P (tProd na ty body)) ->
-(forall (na : aname) (ty body : term),
-(*  expanded Σ ty -> P ty -> *) expanded Σ body -> P body -> P (tLambda na ty body)) ->
-(forall (na : aname) (def def_ty body : term),
- expanded Σ def ->
- P def ->
- (* expanded Σ def_ty -> 
- P def_ty -> *) expanded Σ body -> P body -> P (tLetIn na def def_ty body)) ->
-(forall (f6 : term) (args : list term),
- ~ isConstruct f6 ->
- expanded Σ f6 -> P f6 -> Forall (expanded Σ) args -> Forall P args -> P (mkApps f6 args)) ->
-(forall (c : kername) (u : Instance.t), P (tConst c u)) ->
-(forall (ind : inductive) (u : Instance.t), P (tInd ind u)) ->
-(forall (ci : case_info) (type_info : predicate term) 
+forall (Σ : global_env) (P : list nat -> term -> Prop),
+(forall (Γ : list nat) (n m : nat) (args : list term),
+ nth_error Γ n = Some m ->
+ m <= #|args| -> Forall (expanded Σ Γ) args -> Forall (P Γ) args -> P Γ (mkApps (tRel n) args)) ->
+(forall (Γ : list nat) (id : ident), P Γ (tVar id)) ->
+(forall (Γ : list nat) (ev : nat) (args : list term),
+ Forall (expanded Σ Γ) args -> Forall (P Γ) args -> P Γ (tEvar ev args)) ->
+(forall (Γ : list nat) (s : Universe.t), P Γ (tSort s)) ->
+(forall (Γ : list nat) (na : aname) (ty body : term), P Γ (tProd na ty body)) ->
+(forall (Γ : list nat) (na : aname) (ty body : term),
+ expanded Σ (0 :: Γ) body -> P (0 :: Γ) body -> P Γ (tLambda na ty body)) ->
+(forall (Γ : list nat) (na : aname) (def def_ty body : term),
+ expanded Σ Γ def ->
+ P Γ def ->
+ expanded Σ (0 :: Γ) body ->
+ P (0 :: Γ) body -> P Γ (tLetIn na def def_ty body)) ->
+(forall (Γ : list nat) (f6 : term) (args : list term),
+~ (isConstruct f6 || isFix f6 || isRel f6) ->
+ expanded Σ Γ f6 ->
+ P Γ f6 -> Forall (expanded Σ Γ) args -> Forall (P Γ) args -> P Γ (mkApps f6 args)) ->
+(forall (Γ : list nat) (c : kername) (u : Instance.t), P Γ (tConst c u)) ->
+(forall (Γ : list nat) (ind : inductive) (u : Instance.t), P Γ (tInd ind u)) ->
+(forall (Γ : list nat) (ci : case_info) (type_info : predicate term)
    (discr : term) (branches : list (branch term)),
- expanded Σ discr ->
- P discr ->
- Forall (fun br : branch term => expanded Σ (bbody br)) branches ->
- Forall (fun br : branch term => P (bbody br)) branches ->
- P (tCase ci type_info discr branches)) ->
-(forall (proj : projection) (t : term),
- expanded Σ t -> P t -> P (tProj proj t)) ->
-
- (forall (mfix : mfixpoint term) (idx : nat), 
- Forall (fun d => expanded Σ d.(dtype) /\ expanded Σ d.(dbody)) mfix -> 
- Forall (fun d => P d.(dtype) /\ P d.(dbody)) mfix -> 
- P (tFix mfix idx)) ->
-(forall (mfix : mfixpoint term) (idx : nat), 
- Forall (fun d => expanded Σ d.(dtype) /\ expanded Σ d.(dbody)) mfix -> 
- Forall (fun d => P d.(dtype) /\ P d.(dbody)) mfix -> 
- P (tCoFix mfix idx)) ->
-(forall (ind : inductive) (c : nat) (u : Instance.t)
-   (mind : mutual_inductive_body) (idecl : one_inductive_body)
-   (cdecl : constructor_body) (args : list term),
+ expanded Σ Γ discr ->
+ P Γ discr ->
+ Forall
+   (fun br : branch term =>
+	expanded Σ (repeat 0 #|bcontext br| ++ Γ) (bbody br)) branches ->
+  Forall
+  (fun br : branch term =>
+ P (repeat 0 #|bcontext br| ++ Γ) (bbody br)) branches ->
+ P Γ (tCase ci type_info discr branches)) ->
+(forall (Γ : list nat) (proj : projection) (t : term),
+ expanded Σ Γ t -> P Γ t -> P Γ (tProj proj t)) ->
+(forall (Γ : list nat) (mfix : mfixpoint term) (idx : nat) 
+   (args : list term) (d : def term),
+ Forall
+   (fun d0 : def term =>
+    let ctx := rev_map (fun d1 : def term => 1 + rarg d1) mfix in
+    expanded Σ (ctx ++ Γ) (dbody d0)) mfix ->
+ Forall
+    (fun d0 : def term =>
+     let ctx := rev_map (fun d1 : def term => 1 + rarg d1) mfix in
+     P (ctx ++ Γ) (dbody d0)) mfix ->
+ Forall (expanded Σ Γ) args -> Forall (P Γ) args ->
+ args <> [] ->
+ nth_error mfix idx = Some d ->
+ #|args| > rarg d -> P Γ (mkApps (tFix mfix idx) args)) ->
+(forall (Γ : list nat) (mfix : mfixpoint term) (idx : nat),
+ Forall (fun d : def term => expanded Σ (repeat 0 #|mfix| ++ Γ) (dbody d))
+   mfix ->  Forall (fun d : def term => P (repeat 0 #|mfix| ++ Γ) (dbody d))
+   mfix  -> P Γ (tCoFix mfix idx)) ->
+(forall (Γ : list nat) (ind : inductive) (c : nat) 
+   (u : Instance.t) (mind : mutual_inductive_body)
+   (idecl : one_inductive_body) (cdecl : constructor_body) 
+   (args : list term),
  declared_constructor Σ (ind, c) mind idecl cdecl ->
  #|args| >= ind_npars mind + context_assumptions (cstr_args cdecl) ->
- Forall (expanded Σ) args ->
- Forall P args ->
- P (mkApps (tConstruct ind c u) args)) ->
-forall t : term, expanded Σ t -> P t.
+ Forall (expanded Σ Γ) args -> Forall (P Γ) args -> P Γ (mkApps (tConstruct ind c u) args)) ->
+forall (Γ : list nat) (t : term), expanded Σ Γ t -> P Γ t.
 Proof.
-  intros. revert t H14.
-  fix f 2.
-  intros t Hexp. destruct Hexp; eauto.
-  - eapply H1; eauto. induction H14; econstructor; eauto.
-  - assert (Forall P args) by (induction H15; econstructor; eauto).
-    destruct f0; eauto.
-  - eapply H9; eauto. induction H14; econstructor; eauto.
-  - eapply H11; eauto. induction H14 as [ | ? ? []]; econstructor; cbn in *; eauto; split.
-  - eapply H12; eauto. induction H14 as [ | ? ? []]; econstructor; cbn in *; eauto; split.
-  - eapply H13; eauto. clear - f H16. induction H16; econstructor; cbn in *; eauto; split.
+  intros Σ P HRel HVar HEvar HSort HProd HLamdba HLetIn HApp HConst HInd HCase HProj HFix HCoFix HConstruct.
+  fix f 3.
+  intros Γ t Hexp.  destruct Hexp; eauto.
+  - eapply HRel; eauto. clear - f H0. induction H0; econstructor; eauto.
+  - eapply HEvar; eauto. clear - f H. induction H; econstructor; eauto.
+  - eapply HApp; eauto. clear - f H0. induction H0; econstructor; eauto.
+  - eapply HCase; eauto. induction H; econstructor; eauto.
+  - assert (Forall (P Γ) args). { clear - H0 f. induction H0; econstructor; eauto. }
+    eapply HFix; eauto.
+    revert H. clear - f.
+    generalize mfix at 1 3. intros mfix0 H.  induction H; econstructor; cbn in *; eauto; split.
+  - eapply HCoFix; eauto.
+    revert H. clear - f.
+    generalize mfix at 1 3. intros mfix0 H.  induction H; econstructor; cbn in *; eauto; split.
+  - eapply HConstruct; eauto.
+    clear - H1 f. induction H1; econstructor; eauto.
 Qed.
